Add tests based on Solidity's `yulInterpreterTests`

vc/src/Parser.hs
@@ -1,4 +1,14 @@
 {-# OPTIONS_GHC -w #-}
+{-# LANGUAGE CPP #-}
+{-# LANGUAGE MagicHash #-}
+{-# LANGUAGE BangPatterns #-}
+{-# LANGUAGE TypeSynonymInstances #-}
+{-# LANGUAGE FlexibleInstances #-}
+{-# LANGUAGE PatternGuards #-}
+{-# LANGUAGE NoStrictData #-}
+#if __GLASGOW_HASKELL__ >= 710
+{-# LANGUAGE PartialTypeSignatures #-}
+#endif
 module Parser (calc, lexer) where
 
 import Data.List.NonEmpty (NonEmpty (..), (<|))
@@ -8,1295 +18,993 @@ import Lexer (Token (..), lexer)
 import Types (Identifier, Literal (..), Expr (..), FuncDef' (..), Stmt (..), TopLvlStmt (..), InnerObject (..), Object (..))
 import qualified Data.Array as Happy_Data_Array
 import qualified Data.Bits as Bits
+import qualified GHC.Exts as Happy_GHC_Exts
 import Control.Applicative(Applicative(..))
 import Control.Monad (ap)
 
--- parser produced by Happy Version 1.20.1.1
+-- parser produced by Happy Version 2.0.2
 
-data HappyAbsSyn t4 t5 t6 t7 t8 t9 t10 t11 t12 t13 t14 t15 t16 t17 t18 t19 t20 t21 t22 t23 t24 t25 t26 t27 t28 t29 t30 t31
-	= HappyTerminal (Token)
-	| HappyErrorToken Prelude.Int
-	| HappyAbsSyn4 t4
-	| HappyAbsSyn5 t5
-	| HappyAbsSyn6 t6
-	| HappyAbsSyn7 t7
-	| HappyAbsSyn8 t8
-	| HappyAbsSyn9 t9
-	| HappyAbsSyn10 t10
-	| HappyAbsSyn11 t11
-	| HappyAbsSyn12 t12
-	| HappyAbsSyn13 t13
-	| HappyAbsSyn14 t14
-	| HappyAbsSyn15 t15
-	| HappyAbsSyn16 t16
-	| HappyAbsSyn17 t17
-	| HappyAbsSyn18 t18
-	| HappyAbsSyn19 t19
-	| HappyAbsSyn20 t20
-	| HappyAbsSyn21 t21
-	| HappyAbsSyn22 t22
-	| HappyAbsSyn23 t23
-	| HappyAbsSyn24 t24
-	| HappyAbsSyn25 t25
-	| HappyAbsSyn26 t26
-	| HappyAbsSyn27 t27
-	| HappyAbsSyn28 t28
-	| HappyAbsSyn29 t29
-	| HappyAbsSyn30 t30
-	| HappyAbsSyn31 t31
+data HappyAbsSyn t4 t5 t6 t7 t8 t9 t10 t11 t12 t13 t14 t15 t16 t17 t18 t19 t20 t21 t22 t23 t24 t25 t26 t27 t28 t29 t30 t31 t32
+        = HappyTerminal (Token)
+        | HappyErrorToken Prelude.Int
+        | HappyAbsSyn4 t4
+        | HappyAbsSyn5 t5
+        | HappyAbsSyn6 t6
+        | HappyAbsSyn7 t7
+        | HappyAbsSyn8 t8
+        | HappyAbsSyn9 t9
+        | HappyAbsSyn10 t10
+        | HappyAbsSyn11 t11
+        | HappyAbsSyn12 t12
+        | HappyAbsSyn13 t13
+        | HappyAbsSyn14 t14
+        | HappyAbsSyn15 t15
+        | HappyAbsSyn16 t16
+        | HappyAbsSyn17 t17
+        | HappyAbsSyn18 t18
+        | HappyAbsSyn19 t19
+        | HappyAbsSyn20 t20
+        | HappyAbsSyn21 t21
+        | HappyAbsSyn22 t22
+        | HappyAbsSyn23 t23
+        | HappyAbsSyn24 t24
+        | HappyAbsSyn25 t25
+        | HappyAbsSyn26 t26
+        | HappyAbsSyn27 t27
+        | HappyAbsSyn28 t28
+        | HappyAbsSyn29 t29
+        | HappyAbsSyn30 t30
+        | HappyAbsSyn31 t31
+        | HappyAbsSyn32 t32
 
-happyExpList :: Happy_Data_Array.Array Prelude.Int Prelude.Int
-happyExpList = Happy_Data_Array.listArray (0,250) ([0,0,0,0,0,0,0,0,0,0,32768,2,0,0,0,0,0,0,512,0,0,0,1,0,128,0,0,0,0,256,0,32768,0,0,0,0,0,64,0,0,32768,2,0,8,0,0,0,0,1024,0,0,0,40,0,0,0,0,0,0,0,0,0,1,0,0,0,0,32,0,0,4096,0,0,8,0,0,0,0,16,0,0,0,0,0,33152,32768,1,0,16,0,0,0,0,0,0,0,0,0,0,0,0,0,0,0,0,0,0,0,0,0,0,0,0,0,0,2048,0,0,0,0,0,0,0,0,0,2048,0,0,0,0,0,4,0,0,128,0,0,0,1024,0,8192,0,0,0,384,65511,1,0,0,0,0,0,0,0,0,0,0,0,0,0,0,0,0,0,0,0,0,0,0,0,0,0,0,0,0,0,0,0,0,0,0,0,48,0,0,0,0,0,0,16384,0,0,0,0,0,0,0,0,8,0,0,57344,23,0,0,32256,0,0,8,0,0,0,0,0,0,0,0,0,0,0,0,0,0,1024,0,0,0,64,0,0,8192,0,0,0,16384,0,0,0,0,0,0,0,0,0,0,0,0,0,0,0,0,0,0,64,128,0,0,0,8,0,0,0,1,0,0,2048,0,0,0,256,0,0,36,0,0,34816,0,0,0,16384,0,0,0,0,128,0,0,0,382,0,0,32768,0,0,0,2048,0,0,0,2016,0,0,6144,0,0,8192,0,0,0,128,32768,0,0,0,2016,0,0,48,0,0,0,32768,0,0,0,32256,0,0,0,128,0,0,0,0,0,0,0,0,0,0,0,0,0,0,0,0,0,0,126,0,0,32768,0,0,128,32768,0,0,0,0,0,32768,0,0,0,0,384,0,0,0,0,0,0,0,0,0,0,0,118,0,2048,0,8,0,128,0,0,0,0,0,0,0,0,0,0,0,0,0,0,0,0,0,0,576,0,0,0,0,126,0,0,0,0,0,0,2048,0,0,0,0,0,0,0,8,0,34816,0,0,0,0,2048,0,0,0,256,0,0,1,0,0,0,0,1,0,0,0,0,0,0,128,0,32768,32,0,0,0,0,0,0,0,0,0,0,0,0,0,0,0,382,0,2048,0,0,0,0,0,0,0,8,0,0,32768,0,0,0,0,0,0,0,0,0,0,0,0,0,0,0,0,0,0,2048,0,0,0,16384,0,0,0,0,0,0,0,0,8,0,0,0,0,0,0,0,0,0,0,0,0,0,0,0,0,0,0,0,0,0,0,0,0,520,0,0,0,1,0,0,0,0,0,0,0,0,0,0,0,0,0,0,0,0,0
-	])
+happyExpList :: HappyAddr
+happyExpList = HappyA# "\x00\x00\x00\x00\x00\x00\x00\x00\x00\x00\x00\x00\x00\x00\x00\x00\x00\x00\x00\x00\x00\x00\x14\x00\x00\x00\x00\x00\x00\x00\x00\x00\x00\x00\x00\x00\x00\x40\x00\x00\x00\x00\x00\x00\x40\x00\x00\x00\x00\x40\x00\x00\x00\x00\x00\x00\x00\x00\x00\x00\x01\x00\x00\x00\x00\x01\x00\x00\x00\x00\x00\x00\x00\x00\x00\x00\x01\x00\x00\x00\x00\x00\x00\x14\x00\x00\x00\x80\x00\x00\x00\x00\x00\x00\x00\x00\x00\x00\x80\x00\x00\x00\x00\x00\x00\x00\x0a\x00\x00\x00\x00\x00\x00\x00\x00\x00\x00\x00\x00\x00\x00\x00\x00\x00\x00\x00\x02\x00\x00\x00\x00\x00\x00\x00\x00\x00\x80\x00\x00\x00\x00\x00\x00\x80\x00\x00\x00\x00\x80\x00\x00\x00\x00\x00\x00\x00\x00\x00\x00\x02\x00\x00\x00\x00\x00\x00\x00\x00\x00\x00\x00\xc0\x40\x00\xc0\x00\x00\x00\x00\x10\x00\x00\x00\x00\x00\x00\x00\x00\x00\x00\x00\x00\x00\x00\x00\x00\x00\x00\x00\x00\x00\x00\x00\x00\x00\x00\x00\x00\x00\x00\x00\x00\x00\x00\x00\x00\x00\x00\x00\x00\x00\x00\x00\x00\x00\x00\x00\x00\x00\x00\x00\x00\x00\x00\x00\x04\x00\x00\x00\x00\x00\x00\x00\x00\x00\x00\x00\x00\x00\x00\x00\x00\x00\x00\x00\x20\x00\x00\x00\x00\x00\x00\x00\x00\x00\x00\x20\x00\x00\x00\x00\x00\x00\x08\x00\x00\x00\x00\x00\x00\x00\x80\x00\x00\x00\x00\x08\x00\x00\x00\x00\x00\x00\xc0\x80\xf3\xff\x00\x00\x00\x00\x00\x00\x00\x00\x00\x00\x00\x00\x00\x00\x00\x00\x00\x00\x00\x00\x00\x00\x00\x00\x00\x00\x00\x00\x00\x00\x00\x00\x00\x00\x00\x00\x00\x00\x00\x00\x00\x00\x00\x00\x00\x00\x00\x00\x00\x00\x00\x00\x00\x00\x00\x00\x00\x00\x00\x00\x00\x00\x00\x00\x00\x00\x00\x00\x00\x00\x00\x00\x00\x60\x00\x00\x00\x00\x00\x00\x00\x00\x00\x00\x00\x00\x00\x00\x00\x02\x00\x00\x00\x00\x00\x00\x00\x00\x00\x00\x00\x00\x00\x00\x00\x00\x01\x00\x00\x00\x00\x00\x00\xf8\x05\x00\x00\x00\x00\x00\x00\x3f\x00\x00\x00\x00\x08\x00\x00\x00\x00\x00\x00\x00\x00\x00\x00\x00\x00\x00\x00\x00\x00\x00\x00\x00\x00\x00\x00\x00\x00\x00\x00\x00\x00\x00\x00\x40\x00\x00\x00\x00\x00\x00\x00\x08\x00\x00\x00\x00\x00\x00\x08\x00\x00\x00\x00\x00\x00\x00\x20\x00\x00\x00\x00\x00\x00\x00\x00\x00\x00\x00\x00\x00\x00\x00\x00\x00\x00\x00\x00\x00\x00\x00\x00\x00\x00\x00\x00\x00\x00\x00\x00\x00\x00\x00\x00\x00\x04\x00\x08\x00\x00\x00\x00\x00\x00\x00\x01\x00\x00\x00\x00\x00\x00\x40\x00\x00\x00\x00\x00\x00\x00\x18\x00\x00\x00\x00\x00\x00\x00\x01\x00\x00\x00\x00\x48\x00\x00\x00\x00\x00\x00\x20\x02\x00\x00\x00\x00\x00\x00\x00\x02\x00\x00\x00\x00\x00\x00\x00\x00\x08\x00\x00\x00\x00\x00\x00\xc0\x2f\x00\x00\x00\x00\x00\x00\x20\x00\x00\x00\x00\x00\x00\x00\x04\x00\x00\x00\x00\x00\x00\xe0\x07\x00\x00\x00\x00\x00\x30\x00\x00\x00\x00\x00\x80\x00\x00\x00\x00\x00\x00\x00\x04\x00\x00\x04\x00\x00\x00\x00\x00\x00\x7e\x00\x00\x00\x00\x00\x06\x00\x00\x00\x00\x00\x00\x00\x00\x20\x00\x00\x00\x00\x00\x00\x00\x3f\x00\x00\x00\x00\x00\x00\x80\x00\x00\x00\x00\x00\x00\x00\x00\x00\x00\x00\x00\x00\x00\x00\x00\x00\x00\x00\x00\x00\x00\x00\x00\x00\x00\x00\x00\x00\x00\x00\x00\x00\x00\x00\x00\x00\xc0\x0f\x00\x00\x00\x00\x00\x00\x20\x00\x00\x00\x00\x40\x00\x00\x40\x00\x00\x00\x00\x00\x00\x00\x00\x00\x00\x00\x00\x01\x00\x00\x00\x00\x00\x00\x00\x00\x06\x00\x00\x00\x00\x00\x00\x00\x00\x00\x00\x00\x00\x00\x00\x00\x00\x00\x00\x00\x00\x00\x00\xc0\x0e\x00\x00\x00\x00\x02\x00\x00\x02\x00\x00\x00\x40\x00\x00\x00\x00\x00\x00\x00\x00\x00\x00\x00\x00\x00\x00\x00\x00\x00\x00\x00\x00\x00\x00\x00\x00\x00\x00\x00\x00\x00\x00\x00\x00\x00\x00\x00\x00\x00\x00\x24\x00\x00\x00\x00\x00\x00\x00\x00\xc0\x0f\x00\x00\x00\x00\x00\x00\x00\x00\x00\x00\x00\x00\x00\x00\x04\x00\x00\x00\x00\x00\x00\x00\x00\x00\x00\x00\x00\x00\x00\x10\x00\x00\x00\x00\x20\x02\x00\x00\x00\x00\x00\x00\x00\x00\x80\x01\x00\x00\x00\x00\x01\x00\x00\x00\x00\x00\x00\x00\x00\x00\x00\x00\x00\x00\x00\x00\x00\x00\x00\x00\x00\x00\x00\x00\x00\x00\x00\x00\x00\x00\x10\x00\x00\x00\x00\x00\x00\x00\x00\x00\x00\x00\x00\x00\x00\x00\x00\x00\x02\x00\x00\x00\x00\x04\x01\x00\x00\x00\x00\x00\x00\x00\x00\x00\x00\x00\x00\x00\x00\x00\x00\x00\x00\x00\x00\x00\x00\x00\x00\x00\x00\x00\x00\x00\x00\x00\xbf\x00\x00\x00\x00\x08\x00\x00\x00\x00\x00\x00\x00\x00\x00\x00\x00\x00\x00\x00\x20\x00\x00\x00\x00\x00\x00\x00\x04\x00\x00\x00\x00\x00\x00\x00\x00\x00\x00\x00\x00\x00\x00\x00\x00\x00\x00\x00\x00\x00\x00\x00\x00\x00\x00\x00\x00\x00\x00\x00\x00\x00\x00\x00\x00\x00\x08\x00\x00\x00\x00\x00\x00\x00\x80\x00\x00\x00\x00\x00\x00\x00\x00\x00\x00\x00\x00\x00\x00\x00\x00\x40\x00\x00\x00\x00\x00\x00\x00\x00\x00\x00\x00\x00\x00\x00\x00\x00\x00\x00\x00\x00\x00\x00\x00\x00\x00\x00\x00\x00\x00\x00\x00\x00\x00\x00\x00\x00\x00\x00\x00\x00\x00\x00\x00\x00\x00\x00\x00\x00\x00\x00\x20\x08\x00\x00\x00\x00\x00\x00\x00\x00\x00\x00\x00\x00\x00\x00\x00\x00\x00\x00\x00\x00\x00\x00\x00\x00\x00\x00\x00\x00\x00\x00\x00\x00\x00"#
 
 {-# NOINLINE happyExpListPerState #-}
 happyExpListPerState st =
     token_strs_expected
-  where token_strs = ["error","%dummy","%start_calc","Objects","Object","InnerObject","Code","Block","TopLvlBlock","Statements","TopLvlStmts","TopLvlStmt","Statement","FuncDef","VariableDeclaration","Assignment","Expression","If","Switch","Cases","Case","Default","ForLoop","FunctionCall","ExpressionPrecComment","Arguments","Identifiers","TypeName","TypedIdentifiers","Literal","NumberLiteral","'{'","'}'","'('","')'","'->'","':='","','","':'","function","let","if","switch","case","default","for","break","continue","leave","true","false","ident","str","hex","dec","inlcomment","multicomment","object","code","%eof"]
-        bit_start = st Prelude.* 60
-        bit_end = (st Prelude.+ 1) Prelude.* 60
+  where token_strs = ["error","%dummy","%start_calc","Objects","Object","InnerObject","Code","Block","TopLvlBlock","Statements","TopLvlStmts","TopLvlStmt","Statement","FuncDef","VariableDeclaration","Assignment","Expression","If","Switch","Cases","Case","Default","ForLoop","FunctionCall","ExpressionPrecComment","Arguments","Identifiers","TypeName","TypedIdentifiers","Literal","NumberLiteral","DataLiteral","'{'","'}'","'('","')'","'->'","':='","','","':'","function","let","if","switch","case","default","for","break","continue","leave","true","false","ident","str","hex","dec","inlcomment","multicomment","object","code","%eof"]
+        bit_start = st               Prelude.* 61
+        bit_end   = (st Prelude.+ 1) Prelude.* 61
         read_bit = readArrayBit happyExpList
         bits = Prelude.map read_bit [bit_start..bit_end Prelude.- 1]
-        bits_indexed = Prelude.zip bits [0..59]
+        bits_indexed = Prelude.zip bits [0..60]
         token_strs_expected = Prelude.concatMap f bits_indexed
         f (Prelude.False, _) = []
         f (Prelude.True, nr) = [token_strs Prelude.!! nr]
 
-action_0 (4) = happyGoto action_2
-action_0 _ = happyReduce_1
-
-action_1 _ = happyFail (happyExpListPerState 1)
-
-action_2 (56) = happyShift action_4
-action_2 (58) = happyShift action_5
-action_2 (60) = happyAccept
-action_2 (5) = happyGoto action_3
-action_2 _ = happyFail (happyExpListPerState 2)
-
-action_3 _ = happyReduce_2
-
-action_4 (58) = happyShift action_7
-action_4 _ = happyFail (happyExpListPerState 4)
-
-action_5 (53) = happyShift action_6
-action_5 _ = happyFail (happyExpListPerState 5)
-
-action_6 (32) = happyShift action_9
-action_6 _ = happyFail (happyExpListPerState 6)
-
-action_7 (53) = happyShift action_8
-action_7 _ = happyFail (happyExpListPerState 7)
-
-action_8 (32) = happyShift action_12
-action_8 _ = happyFail (happyExpListPerState 8)
-
-action_9 (59) = happyShift action_11
-action_9 (7) = happyGoto action_10
-action_9 _ = happyFail (happyExpListPerState 9)
-
-action_10 (56) = happyShift action_17
-action_10 (58) = happyShift action_18
-action_10 (6) = happyGoto action_16
-action_10 _ = happyFail (happyExpListPerState 10)
-
-action_11 (32) = happyShift action_15
-action_11 (9) = happyGoto action_14
-action_11 _ = happyFail (happyExpListPerState 11)
-
-action_12 (59) = happyShift action_11
-action_12 (7) = happyGoto action_13
-action_12 _ = happyFail (happyExpListPerState 12)
-
-action_13 (56) = happyShift action_17
-action_13 (58) = happyShift action_18
-action_13 (6) = happyGoto action_23
-action_13 _ = happyFail (happyExpListPerState 13)
-
-action_14 _ = happyReduce_7
-
-action_15 (11) = happyGoto action_22
-action_15 _ = happyReduce_12
-
-action_16 (33) = happyShift action_21
-action_16 _ = happyFail (happyExpListPerState 16)
-
-action_17 (58) = happyShift action_20
-action_17 _ = happyFail (happyExpListPerState 17)
-
-action_18 (53) = happyShift action_19
-action_18 _ = happyFail (happyExpListPerState 18)
-
-action_19 (32) = happyShift action_34
-action_19 _ = happyFail (happyExpListPerState 19)
-
-action_20 (53) = happyShift action_33
-action_20 _ = happyFail (happyExpListPerState 20)
-
-action_21 _ = happyReduce_4
-
-action_22 (32) = happyShift action_28
-action_22 (33) = happyShift action_29
-action_22 (40) = happyShift action_30
-action_22 (56) = happyShift action_31
-action_22 (57) = happyShift action_32
-action_22 (8) = happyGoto action_25
-action_22 (12) = happyGoto action_26
-action_22 (14) = happyGoto action_27
-action_22 _ = happyFail (happyExpListPerState 22)
-
-action_23 (33) = happyShift action_24
-action_23 _ = happyFail (happyExpListPerState 23)
-
-action_24 _ = happyReduce_3
-
-action_25 _ = happyReduce_14
-
-action_26 _ = happyReduce_13
-
-action_27 _ = happyReduce_15
-
-action_28 (10) = happyGoto action_38
-action_28 _ = happyReduce_10
-
-action_29 _ = happyReduce_9
-
-action_30 (52) = happyShift action_37
-action_30 _ = happyFail (happyExpListPerState 30)
-
-action_31 _ = happyReduce_16
-
-action_32 _ = happyReduce_17
-
-action_33 (32) = happyShift action_36
-action_33 _ = happyFail (happyExpListPerState 33)
-
-action_34 (59) = happyShift action_11
-action_34 (7) = happyGoto action_35
-action_34 _ = happyFail (happyExpListPerState 34)
-
-action_35 (52) = happyShift action_69
-action_35 _ = happyFail (happyExpListPerState 35)
-
-action_36 (59) = happyShift action_11
-action_36 (7) = happyGoto action_68
-action_36 _ = happyFail (happyExpListPerState 36)
-
-action_37 (34) = happyShift action_67
-action_37 _ = happyFail (happyExpListPerState 37)
-
-action_38 (32) = happyShift action_28
-action_38 (33) = happyShift action_51
-action_38 (41) = happyShift action_52
-action_38 (42) = happyShift action_53
-action_38 (43) = happyShift action_54
-action_38 (46) = happyShift action_55
-action_38 (47) = happyShift action_56
-action_38 (48) = happyShift action_57
-action_38 (49) = happyShift action_58
-action_38 (50) = happyShift action_59
-action_38 (51) = happyShift action_60
-action_38 (52) = happyShift action_61
-action_38 (53) = happyShift action_62
-action_38 (54) = happyShift action_63
-action_38 (55) = happyShift action_64
-action_38 (56) = happyShift action_65
-action_38 (57) = happyShift action_66
-action_38 (8) = happyGoto action_39
-action_38 (13) = happyGoto action_40
-action_38 (15) = happyGoto action_41
-action_38 (16) = happyGoto action_42
-action_38 (17) = happyGoto action_43
-action_38 (18) = happyGoto action_44
-action_38 (19) = happyGoto action_45
-action_38 (23) = happyGoto action_46
-action_38 (24) = happyGoto action_47
-action_38 (27) = happyGoto action_48
-action_38 (30) = happyGoto action_49
-action_38 (31) = happyGoto action_50
-action_38 _ = happyFail (happyExpListPerState 38)
-
-action_39 _ = happyReduce_18
-
-action_40 _ = happyReduce_11
-
-action_41 _ = happyReduce_19
-
-action_42 _ = happyReduce_20
-
-action_43 _ = happyReduce_22
-
-action_44 _ = happyReduce_21
-
-action_45 _ = happyReduce_23
-
-action_46 _ = happyReduce_24
-
-action_47 _ = happyReduce_37
-
-action_48 (37) = happyShift action_86
-action_48 (38) = happyShift action_87
-action_48 _ = happyFail (happyExpListPerState 48)
-
-action_49 _ = happyReduce_39
-
-action_50 (39) = happyShift action_85
-action_50 _ = happyReduce_66
-
-action_51 _ = happyReduce_8
-
-action_52 (52) = happyShift action_74
-action_52 (29) = happyGoto action_84
-action_52 _ = happyFail (happyExpListPerState 52)
-
-action_53 (50) = happyShift action_59
-action_53 (51) = happyShift action_60
-action_53 (52) = happyShift action_81
-action_53 (53) = happyShift action_62
-action_53 (54) = happyShift action_63
-action_53 (55) = happyShift action_64
-action_53 (57) = happyShift action_83
-action_53 (17) = happyGoto action_82
-action_53 (24) = happyGoto action_47
-action_53 (30) = happyGoto action_49
-action_53 (31) = happyGoto action_50
-action_53 _ = happyFail (happyExpListPerState 53)
-
-action_54 (50) = happyShift action_59
-action_54 (51) = happyShift action_60
-action_54 (52) = happyShift action_81
-action_54 (53) = happyShift action_62
-action_54 (54) = happyShift action_63
-action_54 (55) = happyShift action_64
-action_54 (17) = happyGoto action_80
-action_54 (24) = happyGoto action_47
-action_54 (30) = happyGoto action_49
-action_54 (31) = happyGoto action_50
-action_54 _ = happyFail (happyExpListPerState 54)
-
-action_55 (32) = happyShift action_28
-action_55 (8) = happyGoto action_79
-action_55 _ = happyFail (happyExpListPerState 55)
-
-action_56 _ = happyReduce_26
-
-action_57 _ = happyReduce_25
-
-action_58 _ = happyReduce_27
-
-action_59 (39) = happyShift action_78
-action_59 _ = happyReduce_70
-
-action_60 (39) = happyShift action_77
-action_60 _ = happyReduce_72
-
-action_61 (34) = happyShift action_76
-action_61 (37) = happyReduce_59
-action_61 (38) = happyReduce_59
-action_61 _ = happyReduce_38
-
-action_62 (39) = happyShift action_75
-action_62 _ = happyReduce_68
-
-action_63 _ = happyReduce_74
-
-action_64 _ = happyReduce_75
-
-action_65 _ = happyReduce_28
-
-action_66 _ = happyReduce_29
-
-action_67 (35) = happyShift action_73
-action_67 (52) = happyShift action_74
-action_67 (29) = happyGoto action_72
-action_67 _ = happyFail (happyExpListPerState 67)
-
-action_68 (52) = happyShift action_71
-action_68 _ = happyFail (happyExpListPerState 68)
-
-action_69 (53) = happyShift action_70
-action_69 _ = happyFail (happyExpListPerState 69)
-
-action_70 (52) = happyShift action_115
-action_70 _ = happyFail (happyExpListPerState 70)
-
-action_71 (53) = happyShift action_114
-action_71 _ = happyFail (happyExpListPerState 71)
-
-action_72 (35) = happyShift action_113
-action_72 (38) = happyShift action_93
-action_72 _ = happyFail (happyExpListPerState 72)
-
-action_73 (32) = happyShift action_28
-action_73 (36) = happyShift action_112
-action_73 (8) = happyGoto action_111
-action_73 _ = happyFail (happyExpListPerState 73)
-
-action_74 (39) = happyShift action_110
-action_74 _ = happyReduce_62
-
-action_75 (52) = happyShift action_91
-action_75 (28) = happyGoto action_109
-action_75 _ = happyFail (happyExpListPerState 75)
-
-action_76 (50) = happyShift action_59
-action_76 (51) = happyShift action_60
-action_76 (52) = happyShift action_81
-action_76 (53) = happyShift action_62
-action_76 (54) = happyShift action_63
-action_76 (55) = happyShift action_64
-action_76 (57) = happyShift action_108
-action_76 (17) = happyGoto action_105
-action_76 (24) = happyGoto action_47
-action_76 (25) = happyGoto action_106
-action_76 (26) = happyGoto action_107
-action_76 (30) = happyGoto action_49
-action_76 (31) = happyGoto action_50
-action_76 _ = happyReduce_56
-
-action_77 (52) = happyShift action_91
-action_77 (28) = happyGoto action_104
-action_77 _ = happyFail (happyExpListPerState 77)
-
-action_78 (52) = happyShift action_91
-action_78 (28) = happyGoto action_103
-action_78 _ = happyFail (happyExpListPerState 78)
-
-action_79 (50) = happyShift action_59
-action_79 (51) = happyShift action_60
-action_79 (52) = happyShift action_81
-action_79 (53) = happyShift action_62
-action_79 (54) = happyShift action_63
-action_79 (55) = happyShift action_64
-action_79 (17) = happyGoto action_102
-action_79 (24) = happyGoto action_47
-action_79 (30) = happyGoto action_49
-action_79 (31) = happyGoto action_50
-action_79 _ = happyFail (happyExpListPerState 79)
-
-action_80 (44) = happyShift action_100
-action_80 (45) = happyShift action_101
-action_80 (20) = happyGoto action_97
-action_80 (21) = happyGoto action_98
-action_80 (22) = happyGoto action_99
-action_80 _ = happyFail (happyExpListPerState 80)
-
-action_81 (34) = happyShift action_76
-action_81 _ = happyReduce_38
-
-action_82 (32) = happyShift action_28
-action_82 (56) = happyShift action_96
-action_82 (8) = happyGoto action_95
-action_82 _ = happyFail (happyExpListPerState 82)
-
-action_83 (50) = happyShift action_59
-action_83 (51) = happyShift action_60
-action_83 (52) = happyShift action_81
-action_83 (53) = happyShift action_62
-action_83 (54) = happyShift action_63
-action_83 (55) = happyShift action_64
-action_83 (17) = happyGoto action_94
-action_83 (24) = happyGoto action_47
-action_83 (30) = happyGoto action_49
-action_83 (31) = happyGoto action_50
-action_83 _ = happyFail (happyExpListPerState 83)
-
-action_84 (37) = happyShift action_92
-action_84 (38) = happyShift action_93
-action_84 _ = happyReduce_34
-
-action_85 (52) = happyShift action_91
-action_85 (28) = happyGoto action_90
-action_85 _ = happyFail (happyExpListPerState 85)
-
-action_86 (50) = happyShift action_59
-action_86 (51) = happyShift action_60
-action_86 (52) = happyShift action_81
-action_86 (53) = happyShift action_62
-action_86 (54) = happyShift action_63
-action_86 (55) = happyShift action_64
-action_86 (17) = happyGoto action_89
-action_86 (24) = happyGoto action_47
-action_86 (30) = happyGoto action_49
-action_86 (31) = happyGoto action_50
-action_86 _ = happyFail (happyExpListPerState 86)
-
-action_87 (52) = happyShift action_88
-action_87 _ = happyFail (happyExpListPerState 87)
-
-action_88 _ = happyReduce_60
-
-action_89 _ = happyReduce_36
-
-action_90 _ = happyReduce_67
-
-action_91 _ = happyReduce_61
-
-action_92 (50) = happyShift action_59
-action_92 (51) = happyShift action_60
-action_92 (52) = happyShift action_81
-action_92 (53) = happyShift action_62
-action_92 (54) = happyShift action_63
-action_92 (55) = happyShift action_64
-action_92 (17) = happyGoto action_135
-action_92 (24) = happyGoto action_47
-action_92 (30) = happyGoto action_49
-action_92 (31) = happyGoto action_50
-action_92 _ = happyFail (happyExpListPerState 92)
-
-action_93 (52) = happyShift action_134
-action_93 _ = happyFail (happyExpListPerState 93)
-
-action_94 (32) = happyShift action_28
-action_94 (56) = happyShift action_133
-action_94 (8) = happyGoto action_132
-action_94 _ = happyFail (happyExpListPerState 94)
-
-action_95 _ = happyReduce_40
-
-action_96 (32) = happyShift action_28
-action_96 (8) = happyGoto action_131
-action_96 _ = happyFail (happyExpListPerState 96)
-
-action_97 (44) = happyShift action_100
-action_97 (45) = happyShift action_101
-action_97 (21) = happyGoto action_129
-action_97 (22) = happyGoto action_130
-action_97 _ = happyReduce_44
-
-action_98 _ = happyReduce_47
-
-action_99 _ = happyReduce_46
-
-action_100 (50) = happyShift action_59
-action_100 (51) = happyShift action_60
-action_100 (53) = happyShift action_62
-action_100 (54) = happyShift action_63
-action_100 (55) = happyShift action_64
-action_100 (30) = happyGoto action_128
-action_100 (31) = happyGoto action_50
-action_100 _ = happyFail (happyExpListPerState 100)
-
-action_101 (32) = happyShift action_28
-action_101 (56) = happyShift action_127
-action_101 (8) = happyGoto action_126
-action_101 _ = happyFail (happyExpListPerState 101)
-
-action_102 (32) = happyShift action_28
-action_102 (8) = happyGoto action_125
-action_102 _ = happyFail (happyExpListPerState 102)
-
-action_103 _ = happyReduce_71
-
-action_104 _ = happyReduce_73
-
-action_105 _ = happyReduce_55
-
-action_106 _ = happyReduce_57
-
-action_107 (35) = happyShift action_123
-action_107 (38) = happyShift action_124
-action_107 _ = happyFail (happyExpListPerState 107)
-
-action_108 (50) = happyShift action_59
-action_108 (51) = happyShift action_60
-action_108 (52) = happyShift action_81
-action_108 (53) = happyShift action_62
-action_108 (54) = happyShift action_63
-action_108 (55) = happyShift action_64
-action_108 (17) = happyGoto action_122
-action_108 (24) = happyGoto action_47
-action_108 (30) = happyGoto action_49
-action_108 (31) = happyGoto action_50
-action_108 _ = happyFail (happyExpListPerState 108)
-
-action_109 _ = happyReduce_69
-
-action_110 (52) = happyShift action_91
-action_110 (28) = happyGoto action_121
-action_110 _ = happyFail (happyExpListPerState 110)
-
-action_111 _ = happyReduce_30
-
-action_112 (52) = happyShift action_74
-action_112 (29) = happyGoto action_120
-action_112 _ = happyFail (happyExpListPerState 112)
-
-action_113 (32) = happyShift action_28
-action_113 (36) = happyShift action_119
-action_113 (8) = happyGoto action_118
-action_113 _ = happyFail (happyExpListPerState 113)
-
-action_114 (52) = happyShift action_117
-action_114 _ = happyFail (happyExpListPerState 114)
-
-action_115 (53) = happyShift action_116
-action_115 _ = happyFail (happyExpListPerState 115)
-
-action_116 (33) = happyShift action_145
-action_116 _ = happyFail (happyExpListPerState 116)
-
-action_117 (53) = happyShift action_144
-action_117 _ = happyFail (happyExpListPerState 117)
-
-action_118 _ = happyReduce_31
-
-action_119 (52) = happyShift action_74
-action_119 (29) = happyGoto action_143
-action_119 _ = happyFail (happyExpListPerState 119)
-
-action_120 (32) = happyShift action_28
-action_120 (38) = happyShift action_93
-action_120 (8) = happyGoto action_142
-action_120 _ = happyFail (happyExpListPerState 120)
-
-action_121 _ = happyReduce_63
-
-action_122 _ = happyReduce_54
-
-action_123 _ = happyReduce_53
-
-action_124 (50) = happyShift action_59
-action_124 (51) = happyShift action_60
-action_124 (52) = happyShift action_81
-action_124 (53) = happyShift action_62
-action_124 (54) = happyShift action_63
-action_124 (55) = happyShift action_64
-action_124 (57) = happyShift action_108
-action_124 (17) = happyGoto action_105
-action_124 (24) = happyGoto action_47
-action_124 (25) = happyGoto action_141
-action_124 (30) = happyGoto action_49
-action_124 (31) = happyGoto action_50
-action_124 _ = happyFail (happyExpListPerState 124)
-
-action_125 (32) = happyShift action_28
-action_125 (8) = happyGoto action_140
-action_125 _ = happyFail (happyExpListPerState 125)
-
-action_126 _ = happyReduce_50
-
-action_127 (32) = happyShift action_28
-action_127 (8) = happyGoto action_139
-action_127 _ = happyFail (happyExpListPerState 127)
-
-action_128 (32) = happyShift action_28
-action_128 (8) = happyGoto action_138
-action_128 _ = happyFail (happyExpListPerState 128)
-
-action_129 _ = happyReduce_48
-
-action_130 _ = happyReduce_45
-
-action_131 _ = happyReduce_42
-
-action_132 _ = happyReduce_41
-
-action_133 (32) = happyShift action_28
-action_133 (8) = happyGoto action_137
-action_133 _ = happyFail (happyExpListPerState 133)
-
-action_134 (39) = happyShift action_136
-action_134 _ = happyReduce_64
-
-action_135 _ = happyReduce_35
-
-action_136 (52) = happyShift action_91
-action_136 (28) = happyGoto action_148
-action_136 _ = happyFail (happyExpListPerState 136)
-
-action_137 _ = happyReduce_43
-
-action_138 _ = happyReduce_49
-
-action_139 _ = happyReduce_51
-
-action_140 _ = happyReduce_52
-
-action_141 _ = happyReduce_58
-
-action_142 _ = happyReduce_32
-
-action_143 (32) = happyShift action_28
-action_143 (38) = happyShift action_93
-action_143 (8) = happyGoto action_147
-action_143 _ = happyFail (happyExpListPerState 143)
-
-action_144 (33) = happyShift action_146
-action_144 _ = happyFail (happyExpListPerState 144)
-
-action_145 _ = happyReduce_6
-
-action_146 _ = happyReduce_5
-
-action_147 _ = happyReduce_33
-
-action_148 _ = happyReduce_65
-
-happyReduce_1 = happySpecReduce_0  4 happyReduction_1
+happyActOffsets :: HappyAddr
+happyActOffsets = HappyA# "\x00\x00\x00\x00\x00\x00\x00\x00\x0a\x00\x00\x00\x00\x00\x00\x00\xe6\xff\xff\xff\xf4\xff\xff\xff\x23\x00\x00\x00\x18\x00\x00\x00\x35\x00\x00\x00\x2e\x00\x00\x00\x14\x00\x00\x00\x51\x00\x00\x00\x3f\x00\x00\x00\x14\x00\x00\x00\x00\x00\x00\x00\x00\x00\x00\x00\x6c\x00\x00\x00\x60\x00\x00\x00\x79\x00\x00\x00\x99\x00\x00\x00\x8d\x00\x00\x00\x00\x00\x00\x00\x05\x00\x00\x00\x9d\x00\x00\x00\x00\x00\x00\x00\x00\x00\x00\x00\x00\x00\x00\x00\x00\x00\x00\x00\x00\x00\x00\x00\x00\x00\x00\x00\x8f\x00\x00\x00\x00\x00\x00\x00\x00\x00\x00\x00\x9f\x00\x00\x00\x86\x00\x00\x00\x90\x00\x00\x00\x91\x00\x00\x00\x9e\x00\x00\x00\x01\x00\x00\x00\x00\x00\x00\x00\x00\x00\x00\x00\x00\x00\x00\x00\x00\x00\x00\x00\x00\x00\x00\x00\x00\x00\x00\x00\x00\x00\x00\x00\x00\x00\x00\x00\x00\x00\x00\x00\x8a\x00\x00\x00\x00\x00\x00\x00\xa0\x00\x00\x00\x00\x00\x00\x00\x92\x00\x00\x00\x55\x00\x00\x00\x6a\x00\x00\x00\xa5\x00\x00\x00\x00\x00\x00\x00\x00\x00\x00\x00\x00\x00\x00\x00\xa1\x00\x00\x00\xa2\x00\x00\x00\x5e\x00\x00\x00\xa3\x00\x00\x00\x00\x00\x00\x00\x00\x00\x00\x00\x00\x00\x00\x00\x00\x00\x00\x00\x1e\x00\x00\x00\x97\x00\x00\x00\x98\x00\x00\x00\x62\x00\x00\x00\x9a\x00\x00\x00\x40\x00\x00\x00\x84\x00\x00\x00\xa7\x00\x00\x00\x9c\x00\x00\x00\x5d\x00\x00\x00\x9c\x00\x00\x00\x9c\x00\x00\x00\x6a\x00\x00\x00\x85\x00\x00\x00\xaf\x00\x00\x00\x03\x00\x00\x00\x6a\x00\x00\x00\x8e\x00\x00\x00\xa4\x00\x00\x00\x6a\x00\x00\x00\xa6\x00\x00\x00\x00\x00\x00\x00\x00\x00\x00\x00\x00\x00\x00\x00\x00\x00\x00\x00\x6a\x00\x00\x00\xa8\x00\x00\x00\x04\x00\x00\x00\x00\x00\x00\x00\xb2\x00\x00\x00\x8b\x00\x00\x00\x00\x00\x00\x00\x00\x00\x00\x00\x70\x00\x00\x00\x07\x00\x00\x00\xb2\x00\x00\x00\x00\x00\x00\x00\x00\x00\x00\x00\x00\x00\x00\x00\x00\x00\x00\x00\x56\x00\x00\x00\x6a\x00\x00\x00\x00\x00\x00\x00\xa9\x00\x00\x00\x00\x00\x00\x00\xaa\x00\x00\x00\x89\x00\x00\x00\x80\x00\x00\x00\xb3\x00\x00\x00\x00\x00\x00\x00\x00\x00\x00\x00\x00\x00\x00\x00\xb4\x00\x00\x00\x00\x00\x00\x00\xab\x00\x00\x00\x08\x00\x00\x00\x00\x00\x00\x00\x00\x00\x00\x00\x00\x00\x00\x00\x5d\x00\x00\x00\xb6\x00\x00\x00\x00\x00\x00\x00\xb6\x00\x00\x00\xb6\x00\x00\x00\x00\x00\x00\x00\x00\x00\x00\x00\x00\x00\x00\x00\x00\x00\x00\x00\xb6\x00\x00\x00\xac\x00\x00\x00\x00\x00\x00\x00\xad\x00\x00\x00\x00\x00\x00\x00\x00\x00\x00\x00\x00\x00\x00\x00\x00\x00\x00\x00\x00\x00\x00\x00\x00\x00\x00\x00\x08\x00\x00\x00\x00\x00\x00\x00\x00\x00\x00\x00\x00\x00\x00\x00\x00\x00\x00\x00"#
+
+happyGotoOffsets :: HappyAddr
+happyGotoOffsets = HappyA# "\xb8\x00\x00\x00\x00\x00\x00\x00\xb9\x00\x00\x00\x00\x00\x00\x00\x00\x00\x00\x00\x00\x00\x00\x00\x00\x00\x00\x00\x00\x00\x00\x00\x00\x00\x00\x00\xbe\x00\x00\x00\xba\x00\x00\x00\xbf\x00\x00\x00\xc0\x00\x00\x00\xc3\x00\x00\x00\x00\x00\x00\x00\xc1\x00\x00\x00\x00\x00\x00\x00\x00\x00\x00\x00\x00\x00\x00\x00\x00\x00\x00\x00\x00\x00\x00\x00\x00\x00\x00\x00\x72\x00\x00\x00\x00\x00\x00\x00\x00\x00\x00\x00\x00\x00\x00\x00\x00\x00\x00\x00\x00\x00\x00\x00\xc4\x00\x00\x00\x00\x00\x00\x00\x00\x00\x00\x00\x00\x00\x00\x00\x00\x00\x00\x00\x00\x00\x00\x00\xc6\x00\x00\x00\x00\x00\x00\x00\xc8\x00\x00\x00\x00\x00\x00\x00\x1d\x00\x00\x00\x00\x00\x00\x00\x00\x00\x00\x00\x00\x00\x00\x00\x00\x00\x00\x00\x00\x00\x00\x00\x00\x00\x00\x00\x00\x00\x00\x00\x00\x00\x00\x00\x00\x00\x00\x00\x00\x00\x00\x00\x00\x00\x00\x00\x00\x00\x00\x00\x00\x00\x00\x00\xae\x00\x00\x00\x31\x00\x00\x00\x34\x00\x00\x00\xc2\x00\x00\x00\x00\x00\x00\x00\x00\x00\x00\x00\x00\x00\x00\x00\x00\x00\x00\x00\x00\x00\x00\x00\x00\x00\x00\x00\x00\x00\x00\x00\x00\x00\x00\x00\x00\x00\x00\x00\x00\x00\x00\x00\x00\x00\x00\x00\xb5\x00\x00\x00\x00\x00\x00\x00\x00\x00\x00\x00\xb0\x00\x00\x00\x00\x00\x00\x00\x00\x00\x00\x00\xc9\x00\x00\x00\x00\x00\x00\x00\xb7\x00\x00\x00\x25\x00\x00\x00\xbb\x00\x00\x00\xbc\x00\x00\x00\x39\x00\x00\x00\x7b\x00\x00\x00\x00\x00\x00\x00\xcc\x00\x00\x00\x3c\x00\x00\x00\x00\x00\x00\x00\xbd\x00\x00\x00\x44\x00\x00\x00\x00\x00\x00\x00\x00\x00\x00\x00\x00\x00\x00\x00\x00\x00\x00\x00\x00\x00\x00\x00\x48\x00\x00\x00\x00\x00\x00\x00\xcd\x00\x00\x00\x00\x00\x00\x00\xce\x00\x00\x00\x8c\x00\x00\x00\x00\x00\x00\x00\x00\x00\x00\x00\x81\x00\x00\x00\xd2\x00\x00\x00\xd3\x00\x00\x00\x00\x00\x00\x00\x00\x00\x00\x00\x00\x00\x00\x00\x00\x00\x00\x00\x00\x00\x00\x00\x4c\x00\x00\x00\x00\x00\x00\x00\xc5\x00\x00\x00\x00\x00\x00\x00\xc7\x00\x00\x00\xd4\x00\x00\x00\xca\x00\x00\x00\x00\x00\x00\x00\x00\x00\x00\x00\x00\x00\x00\x00\x00\x00\x00\x00\x00\x00\x00\x00\x00\x00\x00\x00\xcb\x00\x00\x00\xd5\x00\x00\x00\x00\x00\x00\x00\x00\x00\x00\x00\x00\x00\x00\x00\x28\x00\x00\x00\xd6\x00\x00\x00\x00\x00\x00\x00\xd7\x00\x00\x00\xd8\x00\x00\x00\x00\x00\x00\x00\x00\x00\x00\x00\x00\x00\x00\x00\x00\x00\x00\x00\xda\x00\x00\x00\x00\x00\x00\x00\x00\x00\x00\x00\xcf\x00\x00\x00\x00\x00\x00\x00\x00\x00\x00\x00\x00\x00\x00\x00\x00\x00\x00\x00\x00\x00\x00\x00\x00\x00\x00\x00\xdb\x00\x00\x00\x00\x00\x00\x00\x00\x00\x00\x00\x00\x00\x00\x00\x00\x00\x00\x00"#
+
+happyAdjustOffset :: Happy_GHC_Exts.Int# -> Happy_GHC_Exts.Int#
+happyAdjustOffset off = off
+
+happyDefActions :: HappyAddr
+happyDefActions = HappyA# "\xfe\xff\xff\xff\x00\x00\x00\x00\x00\x00\x00\x00\xfd\xff\xff\xff\x00\x00\x00\x00\x00\x00\x00\x00\x00\x00\x00\x00\x00\x00\x00\x00\x00\x00\x00\x00\x00\x00\x00\x00\x00\x00\x00\x00\x00\x00\x00\x00\x00\x00\x00\x00\x00\x00\x00\x00\xf8\xff\xff\xff\xf3\xff\xff\xff\x00\x00\x00\x00\x00\x00\x00\x00\x00\x00\x00\x00\x00\x00\x00\x00\x00\x00\x00\x00\xfb\xff\xff\xff\x00\x00\x00\x00\x00\x00\x00\x00\xfc\xff\xff\xff\xf1\xff\xff\xff\xf2\xff\xff\xff\xf0\xff\xff\xff\xf5\xff\xff\xff\xf6\xff\xff\xff\x00\x00\x00\x00\xef\xff\xff\xff\xee\xff\xff\xff\x00\x00\x00\x00\x00\x00\x00\x00\x00\x00\x00\x00\x00\x00\x00\x00\x00\x00\x00\x00\x00\x00\x00\x00\xed\xff\xff\xff\xf4\xff\xff\xff\xec\xff\xff\xff\xeb\xff\xff\xff\xe9\xff\xff\xff\xea\xff\xff\xff\xe8\xff\xff\xff\xe7\xff\xff\xff\xda\xff\xff\xff\x00\x00\x00\x00\xd8\xff\xff\xff\xbd\xff\xff\xff\xf7\xff\xff\xff\x00\x00\x00\x00\x00\x00\x00\x00\x00\x00\x00\x00\x00\x00\x00\x00\xe5\xff\xff\xff\xe6\xff\xff\xff\xe4\xff\xff\xff\xb9\xff\xff\xff\xb7\xff\xff\xff\xd9\xff\xff\xff\xbb\xff\xff\xff\xb5\xff\xff\xff\xb4\xff\xff\xff\xe3\xff\xff\xff\xe2\xff\xff\xff\x00\x00\x00\x00\x00\x00\x00\x00\x00\x00\x00\x00\x00\x00\x00\x00\x00\x00\x00\x00\x00\x00\x00\x00\x00\x00\x00\x00\xc1\xff\xff\xff\x00\x00\x00\x00\xc7\xff\xff\xff\x00\x00\x00\x00\x00\x00\x00\x00\x00\x00\x00\x00\x00\x00\x00\x00\xd9\xff\xff\xff\x00\x00\x00\x00\x00\x00\x00\x00\xdd\xff\xff\xff\x00\x00\x00\x00\x00\x00\x00\x00\x00\x00\x00\x00\xc3\xff\xff\xff\xdb\xff\xff\xff\xbc\xff\xff\xff\xc2\xff\xff\xff\x00\x00\x00\x00\x00\x00\x00\x00\x00\x00\x00\x00\xd7\xff\xff\xff\x00\x00\x00\x00\xd3\xff\xff\xff\xd0\xff\xff\xff\xd1\xff\xff\xff\x00\x00\x00\x00\x00\x00\x00\x00\x00\x00\x00\x00\xb8\xff\xff\xff\xb6\xff\xff\xff\xc8\xff\xff\xff\xc6\xff\xff\xff\x00\x00\x00\x00\x00\x00\x00\x00\xba\xff\xff\xff\x00\x00\x00\x00\xe1\xff\xff\xff\x00\x00\x00\x00\x00\x00\x00\x00\x00\x00\x00\x00\x00\x00\x00\x00\xb3\xff\xff\xff\xb2\xff\xff\xff\xf9\xff\xff\xff\x00\x00\x00\x00\xe0\xff\xff\xff\x00\x00\x00\x00\x00\x00\x00\x00\xc0\xff\xff\xff\xc9\xff\xff\xff\xca\xff\xff\xff\x00\x00\x00\x00\x00\x00\x00\x00\xcd\xff\xff\xff\x00\x00\x00\x00\x00\x00\x00\x00\xcf\xff\xff\xff\xd2\xff\xff\xff\xd5\xff\xff\xff\xd6\xff\xff\xff\x00\x00\x00\x00\xbf\xff\xff\xff\xdc\xff\xff\xff\x00\x00\x00\x00\xd4\xff\xff\xff\xce\xff\xff\xff\xcc\xff\xff\xff\xcb\xff\xff\xff\xc5\xff\xff\xff\xdf\xff\xff\xff\x00\x00\x00\x00\xfa\xff\xff\xff\xde\xff\xff\xff\xbe\xff\xff\xff"#
+
+happyCheck :: HappyAddr
+happyCheck = HappyA# "\xff\xff\xff\xff\x1b\x00\x00\x00\x01\x00\x00\x00\x02\x00\x00\x00\x01\x00\x00\x00\x01\x00\x00\x00\x01\x00\x00\x00\x02\x00\x00\x00\x01\x00\x00\x00\x01\x00\x00\x00\x16\x00\x00\x00\x0a\x00\x00\x00\x0b\x00\x00\x00\x0c\x00\x00\x00\x09\x00\x00\x00\x07\x00\x00\x00\x0f\x00\x00\x00\x10\x00\x00\x00\x11\x00\x00\x00\x12\x00\x00\x00\x13\x00\x00\x00\x14\x00\x00\x00\x15\x00\x00\x00\x16\x00\x00\x00\x17\x00\x00\x00\x18\x00\x00\x00\x19\x00\x00\x00\x1a\x00\x00\x00\x19\x00\x00\x00\x19\x00\x00\x00\x19\x00\x00\x00\x1a\x00\x00\x00\x19\x00\x00\x00\x04\x00\x00\x00\x04\x00\x00\x00\x19\x00\x00\x00\x01\x00\x00\x00\x1b\x00\x00\x00\x09\x00\x00\x00\x1d\x00\x00\x00\x0b\x00\x00\x00\x0c\x00\x00\x00\x0d\x00\x00\x00\x0e\x00\x00\x00\x0f\x00\x00\x00\x19\x00\x00\x00\x16\x00\x00\x00\x1b\x00\x00\x00\x13\x00\x00\x00\x14\x00\x00\x00\x0d\x00\x00\x00\x15\x00\x00\x00\x17\x00\x00\x00\x0d\x00\x00\x00\x01\x00\x00\x00\x1a\x00\x00\x00\x1b\x00\x00\x00\x14\x00\x00\x00\x15\x00\x00\x00\x16\x00\x00\x00\x14\x00\x00\x00\x15\x00\x00\x00\x0d\x00\x00\x00\x1a\x00\x00\x00\x1b\x00\x00\x00\x0d\x00\x00\x00\x1a\x00\x00\x00\x1b\x00\x00\x00\x04\x00\x00\x00\x14\x00\x00\x00\x0d\x00\x00\x00\x07\x00\x00\x00\x14\x00\x00\x00\x0d\x00\x00\x00\x1c\x00\x00\x00\x1a\x00\x00\x00\x1b\x00\x00\x00\x14\x00\x00\x00\x1a\x00\x00\x00\x1b\x00\x00\x00\x14\x00\x00\x00\x0d\x00\x00\x00\x01\x00\x00\x00\x1a\x00\x00\x00\x1b\x00\x00\x00\x0d\x00\x00\x00\x1a\x00\x00\x00\x1b\x00\x00\x00\x14\x00\x00\x00\x0d\x00\x00\x00\x04\x00\x00\x00\x1c\x00\x00\x00\x14\x00\x00\x00\x07\x00\x00\x00\x1a\x00\x00\x00\x1b\x00\x00\x00\x14\x00\x00\x00\x03\x00\x00\x00\x1a\x00\x00\x00\x1b\x00\x00\x00\x06\x00\x00\x00\x07\x00\x00\x00\x1a\x00\x00\x00\x1b\x00\x00\x00\x13\x00\x00\x00\x14\x00\x00\x00\x15\x00\x00\x00\x16\x00\x00\x00\x17\x00\x00\x00\x18\x00\x00\x00\x02\x00\x00\x00\x1a\x00\x00\x00\x13\x00\x00\x00\x14\x00\x00\x00\x15\x00\x00\x00\x16\x00\x00\x00\x17\x00\x00\x00\x18\x00\x00\x00\x04\x00\x00\x00\x1a\x00\x00\x00\x16\x00\x00\x00\x17\x00\x00\x00\x08\x00\x00\x00\x1b\x00\x00\x00\x0a\x00\x00\x00\x13\x00\x00\x00\x14\x00\x00\x00\x15\x00\x00\x00\x16\x00\x00\x00\x17\x00\x00\x00\x18\x00\x00\x00\x13\x00\x00\x00\x14\x00\x00\x00\x01\x00\x00\x00\x16\x00\x00\x00\x17\x00\x00\x00\x18\x00\x00\x00\x05\x00\x00\x00\x01\x00\x00\x00\x10\x00\x00\x00\x11\x00\x00\x00\x12\x00\x00\x00\x05\x00\x00\x00\x16\x00\x00\x00\x06\x00\x00\x00\x07\x00\x00\x00\x0d\x00\x00\x00\x0e\x00\x00\x00\x06\x00\x00\x00\x07\x00\x00\x00\x16\x00\x00\x00\x17\x00\x00\x00\x0d\x00\x00\x00\x0e\x00\x00\x00\x01\x00\x00\x00\x1a\x00\x00\x00\x1b\x00\x00\x00\x11\x00\x00\x00\x12\x00\x00\x00\x02\x00\x00\x00\x01\x00\x00\x00\x03\x00\x00\x00\x1c\x00\x00\x00\x16\x00\x00\x00\x15\x00\x00\x00\x15\x00\x00\x00\x01\x00\x00\x00\x15\x00\x00\x00\x08\x00\x00\x00\x08\x00\x00\x00\x08\x00\x00\x00\x08\x00\x00\x00\x15\x00\x00\x00\x1c\x00\x00\x00\x16\x00\x00\x00\x08\x00\x00\x00\x16\x00\x00\x00\x15\x00\x00\x00\x03\x00\x00\x00\x01\x00\x00\x00\x08\x00\x00\x00\x02\x00\x00\x00\x02\x00\x00\x00\x01\x00\x00\x00\x00\x00\x00\x00\x15\x00\x00\x00\x01\x00\x00\x00\x15\x00\x00\x00\x02\x00\x00\x00\x15\x00\x00\x00\x15\x00\x00\x00\x15\x00\x00\x00\x15\x00\x00\x00\x03\x00\x00\x00\x15\x00\x00\x00\x03\x00\x00\x00\x05\x00\x00\x00\x02\x00\x00\x00\x04\x00\x00\x00\x19\x00\x00\x00\x07\x00\x00\x00\x03\x00\x00\x00\x06\x00\x00\x00\x03\x00\x00\x00\x1c\x00\x00\x00\x04\x00\x00\x00\x19\x00\x00\x00\x18\x00\x00\x00\x04\x00\x00\x00\x04\x00\x00\x00\x04\x00\x00\x00\x18\x00\x00\x00\x18\x00\x00\x00\x18\x00\x00\x00\x04\x00\x00\x00\x04\x00\x00\x00\x04\x00\x00\x00\x04\x00\x00\x00\x04\x00\x00\x00\x04\x00\x00\x00\x04\x00\x00\x00\x18\x00\x00\x00\x04\x00\x00\x00\x04\x00\x00\x00\x19\x00\x00\x00\xff\xff\xff\xff\xff\xff\xff\xff\xff\xff\xff\xff\x19\x00\x00\x00\xff\xff\xff\xff\x1c\x00\x00\x00\x18\x00\x00\x00\xff\xff\xff\xff\xff\xff\xff\xff\xff\xff\xff\xff\xff\xff\xff\xff\xff\xff\xff\xff\xff\xff\xff\xff\xff\xff\xff\xff\xff\xff\xff\xff\xff\xff\xff\xff\xff\xff\xff\xff\xff\xff\xff\xff\xff\xff\xff\xff\xff\xff\xff\xff\xff\xff\xff\xff\xff\xff\xff\xff\xff\xff\xff\xff\xff\xff\xff\xff"#
+
+happyTable :: HappyAddr
+happyTable = HappyA# "\x00\x00\x00\x00\x08\x00\x00\x00\x1d\x00\x00\x00\x34\x00\x00\x00\x1d\x00\x00\x00\x1d\x00\x00\x00\x1d\x00\x00\x00\x1e\x00\x00\x00\x1d\x00\x00\x00\x1d\x00\x00\x00\x07\x00\x00\x00\x35\x00\x00\x00\x36\x00\x00\x00\x37\x00\x00\x00\x1f\x00\x00\x00\x5e\x00\x00\x00\x38\x00\x00\x00\x39\x00\x00\x00\x3a\x00\x00\x00\x3b\x00\x00\x00\x3c\x00\x00\x00\x3d\x00\x00\x00\x3e\x00\x00\x00\x3f\x00\x00\x00\x40\x00\x00\x00\x41\x00\x00\x00\x42\x00\x00\x00\x43\x00\x00\x00\x61\x00\x00\x00\x88\x00\x00\x00\x20\x00\x00\x00\x21\x00\x00\x00\x82\x00\x00\x00\x27\x00\x00\x00\x4a\x00\x00\x00\x05\x00\x00\x00\x0a\x00\x00\x00\x06\x00\x00\x00\x28\x00\x00\x00\xff\xff\xff\xff\x29\x00\x00\x00\x2a\x00\x00\x00\x2b\x00\x00\x00\x2c\x00\x00\x00\x2d\x00\x00\x00\x12\x00\x00\x00\x09\x00\x00\x00\x13\x00\x00\x00\x2e\x00\x00\x00\x2f\x00\x00\x00\x69\x00\x00\x00\x4b\x00\x00\x00\x30\x00\x00\x00\x69\x00\x00\x00\x0d\x00\x00\x00\x31\x00\x00\x00\x32\x00\x00\x00\x2f\x00\x00\x00\x6a\x00\x00\x00\x6b\x00\x00\x00\x2f\x00\x00\x00\x8f\x00\x00\x00\x52\x00\x00\x00\x31\x00\x00\x00\x32\x00\x00\x00\x50\x00\x00\x00\x31\x00\x00\x00\x32\x00\x00\x00\x72\x00\x00\x00\x2f\x00\x00\x00\x66\x00\x00\x00\x5e\x00\x00\x00\x2f\x00\x00\x00\x5e\x00\x00\x00\x0c\x00\x00\x00\x31\x00\x00\x00\x32\x00\x00\x00\x2f\x00\x00\x00\x31\x00\x00\x00\x32\x00\x00\x00\x2f\x00\x00\x00\x59\x00\x00\x00\x10\x00\x00\x00\x31\x00\x00\x00\x32\x00\x00\x00\x89\x00\x00\x00\x31\x00\x00\x00\x32\x00\x00\x00\x2f\x00\x00\x00\x7c\x00\x00\x00\x7e\x00\x00\x00\x0c\x00\x00\x00\x2f\x00\x00\x00\x7f\x00\x00\x00\x31\x00\x00\x00\x32\x00\x00\x00\x2f\x00\x00\x00\x4d\x00\x00\x00\x31\x00\x00\x00\x32\x00\x00\x00\xc4\xff\xff\xff\xc4\xff\xff\xff\x31\x00\x00\x00\x32\x00\x00\x00\x3c\x00\x00\x00\x3d\x00\x00\x00\x52\x00\x00\x00\x3f\x00\x00\x00\x40\x00\x00\x00\x41\x00\x00\x00\x16\x00\x00\x00\x54\x00\x00\x00\x3c\x00\x00\x00\x3d\x00\x00\x00\x52\x00\x00\x00\x3f\x00\x00\x00\x40\x00\x00\x00\x41\x00\x00\x00\x19\x00\x00\x00\x6d\x00\x00\x00\x75\x00\x00\x00\x76\x00\x00\x00\x1a\x00\x00\x00\x15\x00\x00\x00\x1b\x00\x00\x00\x3c\x00\x00\x00\x3d\x00\x00\x00\x52\x00\x00\x00\x3f\x00\x00\x00\x40\x00\x00\x00\x41\x00\x00\x00\x3c\x00\x00\x00\x3d\x00\x00\x00\x1d\x00\x00\x00\x3f\x00\x00\x00\x40\x00\x00\x00\x41\x00\x00\x00\x71\x00\x00\x00\x1d\x00\x00\x00\x61\x00\x00\x00\x62\x00\x00\x00\x63\x00\x00\x00\x7a\x00\x00\x00\x14\x00\x00\x00\x57\x00\x00\x00\x58\x00\x00\x00\x65\x00\x00\x00\x66\x00\x00\x00\x5d\x00\x00\x00\x5e\x00\x00\x00\x75\x00\x00\x00\x76\x00\x00\x00\x65\x00\x00\x00\x66\x00\x00\x00\x23\x00\x00\x00\x82\x00\x00\x00\x32\x00\x00\x00\x83\x00\x00\x00\x84\x00\x00\x00\x19\x00\x00\x00\x25\x00\x00\x00\x44\x00\x00\x00\x0c\x00\x00\x00\x22\x00\x00\x00\x26\x00\x00\x00\x46\x00\x00\x00\x1d\x00\x00\x00\x4b\x00\x00\x00\x56\x00\x00\x00\x4f\x00\x00\x00\x4e\x00\x00\x00\x4c\x00\x00\x00\x48\x00\x00\x00\x0c\x00\x00\x00\x47\x00\x00\x00\x6f\x00\x00\x00\x73\x00\x00\x00\x5c\x00\x00\x00\x4d\x00\x00\x00\x1d\x00\x00\x00\x8b\x00\x00\x00\x77\x00\x00\x00\x93\x00\x00\x00\x1d\x00\x00\x00\x02\x00\x00\x00\x5c\x00\x00\x00\x03\x00\x00\x00\x59\x00\x00\x00\x10\x00\x00\x00\x89\x00\x00\x00\x5c\x00\x00\x00\x4b\x00\x00\x00\x4b\x00\x00\x00\x0a\x00\x00\x00\x5c\x00\x00\x00\x0d\x00\x00\x00\x0e\x00\x00\x00\x17\x00\x00\x00\x4f\x00\x00\x00\x54\x00\x00\x00\x16\x00\x00\x00\x23\x00\x00\x00\x26\x00\x00\x00\x44\x00\x00\x00\x73\x00\x00\x00\x6f\x00\x00\x00\x48\x00\x00\x00\x6d\x00\x00\x00\x5f\x00\x00\x00\x86\x00\x00\x00\x85\x00\x00\x00\x68\x00\x00\x00\x67\x00\x00\x00\x5a\x00\x00\x00\x80\x00\x00\x00\x7f\x00\x00\x00\x78\x00\x00\x00\x90\x00\x00\x00\x8e\x00\x00\x00\x8d\x00\x00\x00\x8c\x00\x00\x00\x7b\x00\x00\x00\x8b\x00\x00\x00\x93\x00\x00\x00\x7a\x00\x00\x00\x00\x00\x00\x00\x00\x00\x00\x00\x00\x00\x00\x00\x91\x00\x00\x00\x00\x00\x00\x00\x77\x00\x00\x00\x94\x00\x00\x00\x00\x00\x00\x00\x00\x00\x00\x00\x00\x00\x00\x00\x00\x00\x00\x00\x00\x00\x00\x00\x00\x00\x00\x00\x00\x00\x00\x00\x00\x00\x00\x00\x00\x00\x00\x00\x00\x00\x00\x00\x00\x00\x00\x00\x00\x00\x00\x00\x00\x00\x00\x00\x00\x00\x00\x00\x00\x00\x00\x00\x00\x00\x00\x00\x00\x00\x00\x00"#
+
+happyReduceArr = Happy_Data_Array.array (1, 77) [
+        (1 , happyReduce_1),
+        (2 , happyReduce_2),
+        (3 , happyReduce_3),
+        (4 , happyReduce_4),
+        (5 , happyReduce_5),
+        (6 , happyReduce_6),
+        (7 , happyReduce_7),
+        (8 , happyReduce_8),
+        (9 , happyReduce_9),
+        (10 , happyReduce_10),
+        (11 , happyReduce_11),
+        (12 , happyReduce_12),
+        (13 , happyReduce_13),
+        (14 , happyReduce_14),
+        (15 , happyReduce_15),
+        (16 , happyReduce_16),
+        (17 , happyReduce_17),
+        (18 , happyReduce_18),
+        (19 , happyReduce_19),
+        (20 , happyReduce_20),
+        (21 , happyReduce_21),
+        (22 , happyReduce_22),
+        (23 , happyReduce_23),
+        (24 , happyReduce_24),
+        (25 , happyReduce_25),
+        (26 , happyReduce_26),
+        (27 , happyReduce_27),
+        (28 , happyReduce_28),
+        (29 , happyReduce_29),
+        (30 , happyReduce_30),
+        (31 , happyReduce_31),
+        (32 , happyReduce_32),
+        (33 , happyReduce_33),
+        (34 , happyReduce_34),
+        (35 , happyReduce_35),
+        (36 , happyReduce_36),
+        (37 , happyReduce_37),
+        (38 , happyReduce_38),
+        (39 , happyReduce_39),
+        (40 , happyReduce_40),
+        (41 , happyReduce_41),
+        (42 , happyReduce_42),
+        (43 , happyReduce_43),
+        (44 , happyReduce_44),
+        (45 , happyReduce_45),
+        (46 , happyReduce_46),
+        (47 , happyReduce_47),
+        (48 , happyReduce_48),
+        (49 , happyReduce_49),
+        (50 , happyReduce_50),
+        (51 , happyReduce_51),
+        (52 , happyReduce_52),
+        (53 , happyReduce_53),
+        (54 , happyReduce_54),
+        (55 , happyReduce_55),
+        (56 , happyReduce_56),
+        (57 , happyReduce_57),
+        (58 , happyReduce_58),
+        (59 , happyReduce_59),
+        (60 , happyReduce_60),
+        (61 , happyReduce_61),
+        (62 , happyReduce_62),
+        (63 , happyReduce_63),
+        (64 , happyReduce_64),
+        (65 , happyReduce_65),
+        (66 , happyReduce_66),
+        (67 , happyReduce_67),
+        (68 , happyReduce_68),
+        (69 , happyReduce_69),
+        (70 , happyReduce_70),
+        (71 , happyReduce_71),
+        (72 , happyReduce_72),
+        (73 , happyReduce_73),
+        (74 , happyReduce_74),
+        (75 , happyReduce_75),
+        (76 , happyReduce_76),
+        (77 , happyReduce_77)
+        ]
+
+happy_n_terms = 30 :: Prelude.Int
+happy_n_nonterms = 29 :: Prelude.Int
+
+#if __GLASGOW_HASKELL__ >= 710
+#endif
+happyReduce_1 = happySpecReduce_0  0# happyReduction_1
 happyReduction_1  =  HappyAbsSyn4
-		 ([]
-	)
+                 ([]
+        )
 
-happyReduce_2 = happySpecReduce_2  4 happyReduction_2
+#if __GLASGOW_HASKELL__ >= 710
+#endif
+happyReduce_2 = happySpecReduce_2  0# happyReduction_2
 happyReduction_2 (HappyAbsSyn5  happy_var_2)
-	(HappyAbsSyn4  happy_var_1)
-	 =  HappyAbsSyn4
-		 (happy_var_2 : happy_var_1
-	)
+        (HappyAbsSyn4  happy_var_1)
+         =  HappyAbsSyn4
+                 (happy_var_2 : happy_var_1
+        )
 happyReduction_2 _ _  = notHappyAtAll 
 
-happyReduce_3 = happyReduce 7 5 happyReduction_3
+#if __GLASGOW_HASKELL__ >= 710
+#endif
+happyReduce_3 = happyReduce 7# 1# happyReduction_3
 happyReduction_3 (_ `HappyStk`
-	(HappyAbsSyn6  happy_var_6) `HappyStk`
-	(HappyAbsSyn7  happy_var_5) `HappyStk`
-	_ `HappyStk`
-	(HappyTerminal (TokenString happy_var_3)) `HappyStk`
-	_ `HappyStk`
-	(HappyTerminal (TokenInlineComment happy_var_1)) `HappyStk`
-	happyRest)
-	 = HappyAbsSyn5
-		 (Object happy_var_1 happy_var_3 happy_var_5 happy_var_6
-	) `HappyStk` happyRest
+        (HappyAbsSyn6  happy_var_6) `HappyStk`
+        (HappyAbsSyn7  happy_var_5) `HappyStk`
+        _ `HappyStk`
+        (HappyTerminal (TokenString happy_var_3)) `HappyStk`
+        _ `HappyStk`
+        (HappyTerminal (TokenInlineComment happy_var_1)) `HappyStk`
+        happyRest)
+         = HappyAbsSyn5
+                 (Object happy_var_1 happy_var_3 happy_var_5 happy_var_6
+        ) `HappyStk` happyRest
 
-happyReduce_4 = happyReduce 6 5 happyReduction_4
+#if __GLASGOW_HASKELL__ >= 710
+#endif
+happyReduce_4 = happyReduce 6# 1# happyReduction_4
 happyReduction_4 (_ `HappyStk`
-	(HappyAbsSyn6  happy_var_5) `HappyStk`
-	(HappyAbsSyn7  happy_var_4) `HappyStk`
-	_ `HappyStk`
-	(HappyTerminal (TokenString happy_var_2)) `HappyStk`
-	_ `HappyStk`
-	happyRest)
-	 = HappyAbsSyn5
-		 (Object "" happy_var_2 happy_var_4 happy_var_5
-	) `HappyStk` happyRest
+        (HappyAbsSyn6  happy_var_5) `HappyStk`
+        (HappyAbsSyn7  happy_var_4) `HappyStk`
+        _ `HappyStk`
+        (HappyTerminal (TokenString happy_var_2)) `HappyStk`
+        _ `HappyStk`
+        happyRest)
+         = HappyAbsSyn5
+                 (Object "" happy_var_2 happy_var_4 happy_var_5
+        ) `HappyStk` happyRest
 
-happyReduce_5 = happyReduce 10 6 happyReduction_5
+#if __GLASGOW_HASKELL__ >= 710
+#endif
+happyReduce_5 = happyReduce 9# 2# happyReduction_5
 happyReduction_5 (_ `HappyStk`
-	_ `HappyStk`
-	_ `HappyStk`
-	_ `HappyStk`
-	_ `HappyStk`
-	(HappyAbsSyn7  happy_var_5) `HappyStk`
-	_ `HappyStk`
-	(HappyTerminal (TokenString happy_var_3)) `HappyStk`
-	_ `HappyStk`
-	(HappyTerminal (TokenInlineComment happy_var_1)) `HappyStk`
-	happyRest)
-	 = HappyAbsSyn6
-		 (InnerObject happy_var_1 happy_var_3 happy_var_5
-	) `HappyStk` happyRest
+        _ `HappyStk`
+        _ `HappyStk`
+        _ `HappyStk`
+        (HappyAbsSyn7  happy_var_5) `HappyStk`
+        _ `HappyStk`
+        (HappyTerminal (TokenString happy_var_3)) `HappyStk`
+        _ `HappyStk`
+        (HappyTerminal (TokenInlineComment happy_var_1)) `HappyStk`
+        happyRest)
+         = HappyAbsSyn6
+                 (InnerObject happy_var_1 happy_var_3 happy_var_5
+        ) `HappyStk` happyRest
 
-happyReduce_6 = happyReduce 9 6 happyReduction_6
+#if __GLASGOW_HASKELL__ >= 710
+#endif
+happyReduce_6 = happyReduce 8# 2# happyReduction_6
 happyReduction_6 (_ `HappyStk`
-	_ `HappyStk`
-	_ `HappyStk`
-	_ `HappyStk`
-	_ `HappyStk`
-	(HappyAbsSyn7  happy_var_4) `HappyStk`
-	_ `HappyStk`
-	(HappyTerminal (TokenString happy_var_2)) `HappyStk`
-	_ `HappyStk`
-	happyRest)
-	 = HappyAbsSyn6
-		 (InnerObject "" happy_var_2 happy_var_4
-	) `HappyStk` happyRest
+        _ `HappyStk`
+        _ `HappyStk`
+        _ `HappyStk`
+        (HappyAbsSyn7  happy_var_4) `HappyStk`
+        _ `HappyStk`
+        (HappyTerminal (TokenString happy_var_2)) `HappyStk`
+        _ `HappyStk`
+        happyRest)
+         = HappyAbsSyn6
+                 (InnerObject "" happy_var_2 happy_var_4
+        ) `HappyStk` happyRest
 
-happyReduce_7 = happySpecReduce_2  7 happyReduction_7
+#if __GLASGOW_HASKELL__ >= 710
+#endif
+happyReduce_7 = happySpecReduce_2  3# happyReduction_7
 happyReduction_7 (HappyAbsSyn9  happy_var_2)
-	_
-	 =  HappyAbsSyn7
-		 (happy_var_2
-	)
+        _
+         =  HappyAbsSyn7
+                 (happy_var_2
+        )
 happyReduction_7 _ _  = notHappyAtAll 
 
-happyReduce_8 = happySpecReduce_3  8 happyReduction_8
+#if __GLASGOW_HASKELL__ >= 710
+#endif
+happyReduce_8 = happySpecReduce_3  4# happyReduction_8
 happyReduction_8 _
-	(HappyAbsSyn10  happy_var_2)
-	_
-	 =  HappyAbsSyn8
-		 (reverse happy_var_2
-	)
+        (HappyAbsSyn10  happy_var_2)
+        _
+         =  HappyAbsSyn8
+                 (reverse happy_var_2
+        )
 happyReduction_8 _ _ _  = notHappyAtAll 
 
-happyReduce_9 = happySpecReduce_3  9 happyReduction_9
+#if __GLASGOW_HASKELL__ >= 710
+#endif
+happyReduce_9 = happySpecReduce_3  5# happyReduction_9
 happyReduction_9 _
-	(HappyAbsSyn11  happy_var_2)
-	_
-	 =  HappyAbsSyn9
-		 (reverse happy_var_2
-	)
+        (HappyAbsSyn11  happy_var_2)
+        _
+         =  HappyAbsSyn9
+                 (reverse happy_var_2
+        )
 happyReduction_9 _ _ _  = notHappyAtAll 
 
-happyReduce_10 = happySpecReduce_0  10 happyReduction_10
+#if __GLASGOW_HASKELL__ >= 710
+#endif
+happyReduce_10 = happySpecReduce_0  6# happyReduction_10
 happyReduction_10  =  HappyAbsSyn10
-		 ([]
-	)
+                 ([]
+        )
 
-happyReduce_11 = happySpecReduce_2  10 happyReduction_11
+#if __GLASGOW_HASKELL__ >= 710
+#endif
+happyReduce_11 = happySpecReduce_2  6# happyReduction_11
 happyReduction_11 (HappyAbsSyn13  happy_var_2)
-	(HappyAbsSyn10  happy_var_1)
-	 =  HappyAbsSyn10
-		 (happy_var_2 : happy_var_1
-	)
+        (HappyAbsSyn10  happy_var_1)
+         =  HappyAbsSyn10
+                 (happy_var_2 : happy_var_1
+        )
 happyReduction_11 _ _  = notHappyAtAll 
 
-happyReduce_12 = happySpecReduce_0  11 happyReduction_12
+#if __GLASGOW_HASKELL__ >= 710
+#endif
+happyReduce_12 = happySpecReduce_0  7# happyReduction_12
 happyReduction_12  =  HappyAbsSyn11
-		 ([]
-	)
+                 ([]
+        )
 
-happyReduce_13 = happySpecReduce_2  11 happyReduction_13
+#if __GLASGOW_HASKELL__ >= 710
+#endif
+happyReduce_13 = happySpecReduce_2  7# happyReduction_13
 happyReduction_13 (HappyAbsSyn12  happy_var_2)
-	(HappyAbsSyn11  happy_var_1)
-	 =  HappyAbsSyn11
-		 (happy_var_2 : happy_var_1
-	)
+        (HappyAbsSyn11  happy_var_1)
+         =  HappyAbsSyn11
+                 (happy_var_2 : happy_var_1
+        )
 happyReduction_13 _ _  = notHappyAtAll 
 
-happyReduce_14 = happySpecReduce_1  12 happyReduction_14
+#if __GLASGOW_HASKELL__ >= 710
+#endif
+happyReduce_14 = happySpecReduce_1  8# happyReduction_14
 happyReduction_14 _
-	 =  HappyAbsSyn12
-		 (UnusedBlock
-	)
+         =  HappyAbsSyn12
+                 (UnusedBlock
+        )
 
-happyReduce_15 = happySpecReduce_1  12 happyReduction_15
+#if __GLASGOW_HASKELL__ >= 710
+#endif
+happyReduce_15 = happySpecReduce_1  8# happyReduction_15
 happyReduction_15 (HappyAbsSyn14  happy_var_1)
-	 =  HappyAbsSyn12
-		 (FuncDefStmt happy_var_1
-	)
+         =  HappyAbsSyn12
+                 (FuncDefStmt happy_var_1
+        )
 happyReduction_15 _  = notHappyAtAll 
 
-happyReduce_16 = happySpecReduce_1  12 happyReduction_16
+#if __GLASGOW_HASKELL__ >= 710
+#endif
+happyReduce_16 = happySpecReduce_1  8# happyReduction_16
 happyReduction_16 _
-	 =  HappyAbsSyn12
-		 (UnusedBlock
-	)
+         =  HappyAbsSyn12
+                 (UnusedBlock
+        )
 
-happyReduce_17 = happySpecReduce_1  12 happyReduction_17
+#if __GLASGOW_HASKELL__ >= 710
+#endif
+happyReduce_17 = happySpecReduce_1  8# happyReduction_17
 happyReduction_17 _
-	 =  HappyAbsSyn12
-		 (UnusedBlock
-	)
+         =  HappyAbsSyn12
+                 (UnusedBlock
+        )
 
-happyReduce_18 = happySpecReduce_1  13 happyReduction_18
+#if __GLASGOW_HASKELL__ >= 710
+#endif
+happyReduce_18 = happySpecReduce_1  9# happyReduction_18
 happyReduction_18 (HappyAbsSyn8  happy_var_1)
-	 =  HappyAbsSyn13
-		 (Block happy_var_1
-	)
+         =  HappyAbsSyn13
+                 (Block happy_var_1
+        )
 happyReduction_18 _  = notHappyAtAll 
 
-happyReduce_19 = happySpecReduce_1  13 happyReduction_19
+#if __GLASGOW_HASKELL__ >= 710
+#endif
+happyReduce_19 = happySpecReduce_1  9# happyReduction_19
 happyReduction_19 (HappyAbsSyn15  happy_var_1)
-	 =  HappyAbsSyn13
-		 (let (idens, mbExpr) = happy_var_1 in
+         =  HappyAbsSyn13
+                 (let (idens, mbExpr) = happy_var_1 in
                                                 case mbExpr of
                                                   Just expr -> LetInit idens expr
                                                   Nothing   -> Declaration idens
-	)
+        )
 happyReduction_19 _  = notHappyAtAll 
 
-happyReduce_20 = happySpecReduce_1  13 happyReduction_20
+#if __GLASGOW_HASKELL__ >= 710
+#endif
+happyReduce_20 = happySpecReduce_1  9# happyReduction_20
 happyReduction_20 (HappyAbsSyn16  happy_var_1)
-	 =  HappyAbsSyn13
-		 ((uncurry Assignment) happy_var_1
-	)
+         =  HappyAbsSyn13
+                 ((uncurry Assignment) happy_var_1
+        )
 happyReduction_20 _  = notHappyAtAll 
 
-happyReduce_21 = happySpecReduce_1  13 happyReduction_21
+#if __GLASGOW_HASKELL__ >= 710
+#endif
+happyReduce_21 = happySpecReduce_1  9# happyReduction_21
 happyReduction_21 (HappyAbsSyn18  happy_var_1)
-	 =  HappyAbsSyn13
-		 ((uncurry If) happy_var_1
-	)
+         =  HappyAbsSyn13
+                 ((uncurry If) happy_var_1
+        )
 happyReduction_21 _  = notHappyAtAll 
 
-happyReduce_22 = happySpecReduce_1  13 happyReduction_22
+#if __GLASGOW_HASKELL__ >= 710
+#endif
+happyReduce_22 = happySpecReduce_1  9# happyReduction_22
 happyReduction_22 (HappyAbsSyn17  happy_var_1)
-	 =  HappyAbsSyn13
-		 (ExpressionStmt happy_var_1
-	)
+         =  HappyAbsSyn13
+                 (ExpressionStmt happy_var_1
+        )
 happyReduction_22 _  = notHappyAtAll 
 
-happyReduce_23 = happySpecReduce_1  13 happyReduction_23
+#if __GLASGOW_HASKELL__ >= 710
+#endif
+happyReduce_23 = happySpecReduce_1  9# happyReduction_23
 happyReduction_23 (HappyAbsSyn19  happy_var_1)
-	 =  HappyAbsSyn13
-		 ((uncurry3 Switch) happy_var_1
-	)
+         =  HappyAbsSyn13
+                 ((uncurry3 Switch) happy_var_1
+        )
 happyReduction_23 _  = notHappyAtAll 
 
-happyReduce_24 = happySpecReduce_1  13 happyReduction_24
+#if __GLASGOW_HASKELL__ >= 710
+#endif
+happyReduce_24 = happySpecReduce_1  9# happyReduction_24
 happyReduction_24 (HappyAbsSyn23  happy_var_1)
-	 =  HappyAbsSyn13
-		 ((uncurry4 For) happy_var_1
-	)
+         =  HappyAbsSyn13
+                 ((uncurry4 For) happy_var_1
+        )
 happyReduction_24 _  = notHappyAtAll 
 
-happyReduce_25 = happySpecReduce_1  13 happyReduction_25
+#if __GLASGOW_HASKELL__ >= 710
+#endif
+happyReduce_25 = happySpecReduce_1  9# happyReduction_25
 happyReduction_25 _
-	 =  HappyAbsSyn13
-		 (Continue
-	)
+         =  HappyAbsSyn13
+                 (Continue
+        )
 
-happyReduce_26 = happySpecReduce_1  13 happyReduction_26
+#if __GLASGOW_HASKELL__ >= 710
+#endif
+happyReduce_26 = happySpecReduce_1  9# happyReduction_26
 happyReduction_26 _
-	 =  HappyAbsSyn13
-		 (Break
-	)
+         =  HappyAbsSyn13
+                 (Break
+        )
 
-happyReduce_27 = happySpecReduce_1  13 happyReduction_27
+#if __GLASGOW_HASKELL__ >= 710
+#endif
+happyReduce_27 = happySpecReduce_1  9# happyReduction_27
 happyReduction_27 _
-	 =  HappyAbsSyn13
-		 (Leave
-	)
+         =  HappyAbsSyn13
+                 (Leave
+        )
 
-happyReduce_28 = happySpecReduce_1  13 happyReduction_28
+#if __GLASGOW_HASKELL__ >= 710
+#endif
+happyReduce_28 = happySpecReduce_1  9# happyReduction_28
 happyReduction_28 (HappyTerminal (TokenInlineComment happy_var_1))
-	 =  HappyAbsSyn13
-		 (InlineComment happy_var_1
-	)
+         =  HappyAbsSyn13
+                 (InlineComment happy_var_1
+        )
 happyReduction_28 _  = notHappyAtAll 
 
-happyReduce_29 = happySpecReduce_1  13 happyReduction_29
+#if __GLASGOW_HASKELL__ >= 710
+#endif
+happyReduce_29 = happySpecReduce_1  9# happyReduction_29
 happyReduction_29 (HappyTerminal (TokenMultilineComment happy_var_1))
-	 =  HappyAbsSyn13
-		 (MultilineComment happy_var_1
-	)
+         =  HappyAbsSyn13
+                 (MultilineComment happy_var_1
+        )
 happyReduction_29 _  = notHappyAtAll 
 
-happyReduce_30 = happyReduce 5 14 happyReduction_30
+#if __GLASGOW_HASKELL__ >= 710
+#endif
+happyReduce_30 = happyReduce 5# 10# happyReduction_30
 happyReduction_30 ((HappyAbsSyn8  happy_var_5) `HappyStk`
-	_ `HappyStk`
-	_ `HappyStk`
-	(HappyTerminal (TokenIdentifier happy_var_2)) `HappyStk`
-	_ `HappyStk`
-	happyRest)
-	 = HappyAbsSyn14
-		 (FuncDef' happy_var_2 [] [] happy_var_5
-	) `HappyStk` happyRest
+        _ `HappyStk`
+        _ `HappyStk`
+        (HappyTerminal (TokenIdentifier happy_var_2)) `HappyStk`
+        _ `HappyStk`
+        happyRest)
+         = HappyAbsSyn14
+                 (FuncDef' happy_var_2 [] [] happy_var_5
+        ) `HappyStk` happyRest
 
-happyReduce_31 = happyReduce 6 14 happyReduction_31
+#if __GLASGOW_HASKELL__ >= 710
+#endif
+happyReduce_31 = happyReduce 6# 10# happyReduction_31
 happyReduction_31 ((HappyAbsSyn8  happy_var_6) `HappyStk`
-	_ `HappyStk`
-	(HappyAbsSyn29  happy_var_4) `HappyStk`
-	_ `HappyStk`
-	(HappyTerminal (TokenIdentifier happy_var_2)) `HappyStk`
-	_ `HappyStk`
-	happyRest)
-	 = HappyAbsSyn14
-		 (FuncDef' happy_var_2 (reverse (NE.toList happy_var_4)) [] happy_var_6
-	) `HappyStk` happyRest
+        _ `HappyStk`
+        (HappyAbsSyn29  happy_var_4) `HappyStk`
+        _ `HappyStk`
+        (HappyTerminal (TokenIdentifier happy_var_2)) `HappyStk`
+        _ `HappyStk`
+        happyRest)
+         = HappyAbsSyn14
+                 (FuncDef' happy_var_2 (reverse (NE.toList happy_var_4)) [] happy_var_6
+        ) `HappyStk` happyRest
 
-happyReduce_32 = happyReduce 7 14 happyReduction_32
+#if __GLASGOW_HASKELL__ >= 710
+#endif
+happyReduce_32 = happyReduce 7# 10# happyReduction_32
 happyReduction_32 ((HappyAbsSyn8  happy_var_7) `HappyStk`
-	(HappyAbsSyn29  happy_var_6) `HappyStk`
-	_ `HappyStk`
-	_ `HappyStk`
-	_ `HappyStk`
-	(HappyTerminal (TokenIdentifier happy_var_2)) `HappyStk`
-	_ `HappyStk`
-	happyRest)
-	 = HappyAbsSyn14
-		 (FuncDef' happy_var_2 [] (reverse (NE.toList happy_var_6)) happy_var_7
-	) `HappyStk` happyRest
+        (HappyAbsSyn29  happy_var_6) `HappyStk`
+        _ `HappyStk`
+        _ `HappyStk`
+        _ `HappyStk`
+        (HappyTerminal (TokenIdentifier happy_var_2)) `HappyStk`
+        _ `HappyStk`
+        happyRest)
+         = HappyAbsSyn14
+                 (FuncDef' happy_var_2 [] (reverse (NE.toList happy_var_6)) happy_var_7
+        ) `HappyStk` happyRest
 
-happyReduce_33 = happyReduce 8 14 happyReduction_33
+#if __GLASGOW_HASKELL__ >= 710
+#endif
+happyReduce_33 = happyReduce 8# 10# happyReduction_33
 happyReduction_33 ((HappyAbsSyn8  happy_var_8) `HappyStk`
-	(HappyAbsSyn29  happy_var_7) `HappyStk`
-	_ `HappyStk`
-	_ `HappyStk`
-	(HappyAbsSyn29  happy_var_4) `HappyStk`
-	_ `HappyStk`
-	(HappyTerminal (TokenIdentifier happy_var_2)) `HappyStk`
-	_ `HappyStk`
-	happyRest)
-	 = HappyAbsSyn14
-		 (FuncDef' happy_var_2 (reverse (NE.toList happy_var_4)) (reverse (NE.toList happy_var_7)) happy_var_8
-	) `HappyStk` happyRest
+        (HappyAbsSyn29  happy_var_7) `HappyStk`
+        _ `HappyStk`
+        _ `HappyStk`
+        (HappyAbsSyn29  happy_var_4) `HappyStk`
+        _ `HappyStk`
+        (HappyTerminal (TokenIdentifier happy_var_2)) `HappyStk`
+        _ `HappyStk`
+        happyRest)
+         = HappyAbsSyn14
+                 (FuncDef' happy_var_2 (reverse (NE.toList happy_var_4)) (reverse (NE.toList happy_var_7)) happy_var_8
+        ) `HappyStk` happyRest
 
-happyReduce_34 = happySpecReduce_2  15 happyReduction_34
+#if __GLASGOW_HASKELL__ >= 710
+#endif
+happyReduce_34 = happySpecReduce_2  11# happyReduction_34
 happyReduction_34 (HappyAbsSyn29  happy_var_2)
-	_
-	 =  HappyAbsSyn15
-		 ((NE.reverse happy_var_2, Nothing)
-	)
+        _
+         =  HappyAbsSyn15
+                 ((NE.reverse happy_var_2, Nothing)
+        )
 happyReduction_34 _ _  = notHappyAtAll 
 
-happyReduce_35 = happyReduce 4 15 happyReduction_35
+#if __GLASGOW_HASKELL__ >= 710
+#endif
+happyReduce_35 = happyReduce 4# 11# happyReduction_35
 happyReduction_35 ((HappyAbsSyn17  happy_var_4) `HappyStk`
-	_ `HappyStk`
-	(HappyAbsSyn29  happy_var_2) `HappyStk`
-	_ `HappyStk`
-	happyRest)
-	 = HappyAbsSyn15
-		 ((NE.reverse happy_var_2, Just happy_var_4)
-	) `HappyStk` happyRest
+        _ `HappyStk`
+        (HappyAbsSyn29  happy_var_2) `HappyStk`
+        _ `HappyStk`
+        happyRest)
+         = HappyAbsSyn15
+                 ((NE.reverse happy_var_2, Just happy_var_4)
+        ) `HappyStk` happyRest
 
-happyReduce_36 = happySpecReduce_3  16 happyReduction_36
+#if __GLASGOW_HASKELL__ >= 710
+#endif
+happyReduce_36 = happySpecReduce_3  12# happyReduction_36
 happyReduction_36 (HappyAbsSyn17  happy_var_3)
-	_
-	(HappyAbsSyn27  happy_var_1)
-	 =  HappyAbsSyn16
-		 ((NE.reverse happy_var_1, happy_var_3)
-	)
+        _
+        (HappyAbsSyn27  happy_var_1)
+         =  HappyAbsSyn16
+                 ((NE.reverse happy_var_1, happy_var_3)
+        )
 happyReduction_36 _ _ _  = notHappyAtAll 
 
-happyReduce_37 = happySpecReduce_1  17 happyReduction_37
+#if __GLASGOW_HASKELL__ >= 710
+#endif
+happyReduce_37 = happySpecReduce_1  13# happyReduction_37
 happyReduction_37 (HappyAbsSyn24  happy_var_1)
-	 =  HappyAbsSyn17
-		 ((uncurry Call) happy_var_1
-	)
+         =  HappyAbsSyn17
+                 ((uncurry Call) happy_var_1
+        )
 happyReduction_37 _  = notHappyAtAll 
 
-happyReduce_38 = happySpecReduce_1  17 happyReduction_38
+#if __GLASGOW_HASKELL__ >= 710
+#endif
+happyReduce_38 = happySpecReduce_1  13# happyReduction_38
 happyReduction_38 (HappyTerminal (TokenIdentifier happy_var_1))
-	 =  HappyAbsSyn17
-		 (Var happy_var_1
-	)
+         =  HappyAbsSyn17
+                 (Var happy_var_1
+        )
 happyReduction_38 _  = notHappyAtAll 
 
-happyReduce_39 = happySpecReduce_1  17 happyReduction_39
+#if __GLASGOW_HASKELL__ >= 710
+#endif
+happyReduce_39 = happySpecReduce_1  13# happyReduction_39
 happyReduction_39 (HappyAbsSyn30  happy_var_1)
-	 =  HappyAbsSyn17
-		 (Lit happy_var_1
-	)
+         =  HappyAbsSyn17
+                 (Lit happy_var_1
+        )
 happyReduction_39 _  = notHappyAtAll 
 
-happyReduce_40 = happySpecReduce_3  18 happyReduction_40
+#if __GLASGOW_HASKELL__ >= 710
+#endif
+happyReduce_40 = happySpecReduce_3  14# happyReduction_40
 happyReduction_40 (HappyAbsSyn8  happy_var_3)
-	(HappyAbsSyn17  happy_var_2)
-	_
-	 =  HappyAbsSyn18
-		 ((happy_var_2, happy_var_3)
-	)
+        (HappyAbsSyn17  happy_var_2)
+        _
+         =  HappyAbsSyn18
+                 ((happy_var_2, happy_var_3)
+        )
 happyReduction_40 _ _ _  = notHappyAtAll 
 
-happyReduce_41 = happyReduce 4 18 happyReduction_41
+#if __GLASGOW_HASKELL__ >= 710
+#endif
+happyReduce_41 = happyReduce 4# 14# happyReduction_41
 happyReduction_41 ((HappyAbsSyn8  happy_var_4) `HappyStk`
-	(HappyAbsSyn17  happy_var_3) `HappyStk`
-	_ `HappyStk`
-	_ `HappyStk`
-	happyRest)
-	 = HappyAbsSyn18
-		 ((happy_var_3, happy_var_4)
-	) `HappyStk` happyRest
+        (HappyAbsSyn17  happy_var_3) `HappyStk`
+        _ `HappyStk`
+        _ `HappyStk`
+        happyRest)
+         = HappyAbsSyn18
+                 ((happy_var_3, happy_var_4)
+        ) `HappyStk` happyRest
 
-happyReduce_42 = happyReduce 4 18 happyReduction_42
+#if __GLASGOW_HASKELL__ >= 710
+#endif
+happyReduce_42 = happyReduce 4# 14# happyReduction_42
 happyReduction_42 ((HappyAbsSyn8  happy_var_4) `HappyStk`
-	_ `HappyStk`
-	(HappyAbsSyn17  happy_var_2) `HappyStk`
-	_ `HappyStk`
-	happyRest)
-	 = HappyAbsSyn18
-		 ((happy_var_2, happy_var_4)
-	) `HappyStk` happyRest
+        _ `HappyStk`
+        (HappyAbsSyn17  happy_var_2) `HappyStk`
+        _ `HappyStk`
+        happyRest)
+         = HappyAbsSyn18
+                 ((happy_var_2, happy_var_4)
+        ) `HappyStk` happyRest
 
-happyReduce_43 = happyReduce 5 18 happyReduction_43
+#if __GLASGOW_HASKELL__ >= 710
+#endif
+happyReduce_43 = happyReduce 5# 14# happyReduction_43
 happyReduction_43 ((HappyAbsSyn8  happy_var_5) `HappyStk`
-	_ `HappyStk`
-	(HappyAbsSyn17  happy_var_3) `HappyStk`
-	_ `HappyStk`
-	_ `HappyStk`
-	happyRest)
-	 = HappyAbsSyn18
-		 ((happy_var_3, happy_var_5)
-	) `HappyStk` happyRest
+        _ `HappyStk`
+        (HappyAbsSyn17  happy_var_3) `HappyStk`
+        _ `HappyStk`
+        _ `HappyStk`
+        happyRest)
+         = HappyAbsSyn18
+                 ((happy_var_3, happy_var_5)
+        ) `HappyStk` happyRest
 
-happyReduce_44 = happySpecReduce_3  19 happyReduction_44
+#if __GLASGOW_HASKELL__ >= 710
+#endif
+happyReduce_44 = happySpecReduce_3  15# happyReduction_44
 happyReduction_44 (HappyAbsSyn20  happy_var_3)
-	(HappyAbsSyn17  happy_var_2)
-	_
-	 =  HappyAbsSyn19
-		 ((happy_var_2, reverse happy_var_3, [])
-	)
+        (HappyAbsSyn17  happy_var_2)
+        _
+         =  HappyAbsSyn19
+                 ((happy_var_2, reverse happy_var_3, [])
+        )
 happyReduction_44 _ _ _  = notHappyAtAll 
 
-happyReduce_45 = happyReduce 4 19 happyReduction_45
+#if __GLASGOW_HASKELL__ >= 710
+#endif
+happyReduce_45 = happyReduce 4# 15# happyReduction_45
 happyReduction_45 ((HappyAbsSyn22  happy_var_4) `HappyStk`
-	(HappyAbsSyn20  happy_var_3) `HappyStk`
-	(HappyAbsSyn17  happy_var_2) `HappyStk`
-	_ `HappyStk`
-	happyRest)
-	 = HappyAbsSyn19
-		 ((happy_var_2, reverse happy_var_3, happy_var_4)
-	) `HappyStk` happyRest
+        (HappyAbsSyn20  happy_var_3) `HappyStk`
+        (HappyAbsSyn17  happy_var_2) `HappyStk`
+        _ `HappyStk`
+        happyRest)
+         = HappyAbsSyn19
+                 ((happy_var_2, reverse happy_var_3, happy_var_4)
+        ) `HappyStk` happyRest
 
-happyReduce_46 = happySpecReduce_3  19 happyReduction_46
+#if __GLASGOW_HASKELL__ >= 710
+#endif
+happyReduce_46 = happySpecReduce_3  15# happyReduction_46
 happyReduction_46 (HappyAbsSyn22  happy_var_3)
-	(HappyAbsSyn17  happy_var_2)
-	_
-	 =  HappyAbsSyn19
-		 ((happy_var_2, [],         happy_var_3)
-	)
+        (HappyAbsSyn17  happy_var_2)
+        _
+         =  HappyAbsSyn19
+                 ((happy_var_2, [],         happy_var_3)
+        )
 happyReduction_46 _ _ _  = notHappyAtAll 
 
-happyReduce_47 = happySpecReduce_1  20 happyReduction_47
+#if __GLASGOW_HASKELL__ >= 710
+#endif
+happyReduce_47 = happySpecReduce_1  16# happyReduction_47
 happyReduction_47 (HappyAbsSyn21  happy_var_1)
-	 =  HappyAbsSyn20
-		 ([happy_var_1]
-	)
+         =  HappyAbsSyn20
+                 ([happy_var_1]
+        )
 happyReduction_47 _  = notHappyAtAll 
 
-happyReduce_48 = happySpecReduce_2  20 happyReduction_48
+#if __GLASGOW_HASKELL__ >= 710
+#endif
+happyReduce_48 = happySpecReduce_2  16# happyReduction_48
 happyReduction_48 (HappyAbsSyn21  happy_var_2)
-	(HappyAbsSyn20  happy_var_1)
-	 =  HappyAbsSyn20
-		 (happy_var_2 : happy_var_1
-	)
+        (HappyAbsSyn20  happy_var_1)
+         =  HappyAbsSyn20
+                 (happy_var_2 : happy_var_1
+        )
 happyReduction_48 _ _  = notHappyAtAll 
 
-happyReduce_49 = happySpecReduce_3  21 happyReduction_49
+#if __GLASGOW_HASKELL__ >= 710
+#endif
+happyReduce_49 = happySpecReduce_3  17# happyReduction_49
 happyReduction_49 (HappyAbsSyn8  happy_var_3)
-	(HappyAbsSyn30  happy_var_2)
-	_
-	 =  HappyAbsSyn21
-		 ((happy_var_2, happy_var_3)
-	)
+        (HappyAbsSyn30  happy_var_2)
+        _
+         =  HappyAbsSyn21
+                 ((happy_var_2, happy_var_3)
+        )
 happyReduction_49 _ _ _  = notHappyAtAll 
 
-happyReduce_50 = happySpecReduce_2  22 happyReduction_50
+#if __GLASGOW_HASKELL__ >= 710
+#endif
+happyReduce_50 = happySpecReduce_2  18# happyReduction_50
 happyReduction_50 (HappyAbsSyn8  happy_var_2)
-	_
-	 =  HappyAbsSyn22
-		 (happy_var_2
-	)
+        _
+         =  HappyAbsSyn22
+                 (happy_var_2
+        )
 happyReduction_50 _ _  = notHappyAtAll 
 
-happyReduce_51 = happySpecReduce_3  22 happyReduction_51
+#if __GLASGOW_HASKELL__ >= 710
+#endif
+happyReduce_51 = happySpecReduce_3  18# happyReduction_51
 happyReduction_51 (HappyAbsSyn8  happy_var_3)
-	_
-	_
-	 =  HappyAbsSyn22
-		 (happy_var_3
-	)
+        _
+        _
+         =  HappyAbsSyn22
+                 (happy_var_3
+        )
 happyReduction_51 _ _ _  = notHappyAtAll 
 
-happyReduce_52 = happyReduce 5 23 happyReduction_52
+#if __GLASGOW_HASKELL__ >= 710
+#endif
+happyReduce_52 = happyReduce 5# 19# happyReduction_52
 happyReduction_52 ((HappyAbsSyn8  happy_var_5) `HappyStk`
-	(HappyAbsSyn8  happy_var_4) `HappyStk`
-	(HappyAbsSyn17  happy_var_3) `HappyStk`
-	(HappyAbsSyn8  happy_var_2) `HappyStk`
-	_ `HappyStk`
-	happyRest)
-	 = HappyAbsSyn23
-		 ((happy_var_2, happy_var_3, happy_var_4, happy_var_5)
-	) `HappyStk` happyRest
+        (HappyAbsSyn8  happy_var_4) `HappyStk`
+        (HappyAbsSyn17  happy_var_3) `HappyStk`
+        (HappyAbsSyn8  happy_var_2) `HappyStk`
+        _ `HappyStk`
+        happyRest)
+         = HappyAbsSyn23
+                 ((happy_var_2, happy_var_3, happy_var_4, happy_var_5)
+        ) `HappyStk` happyRest
 
-happyReduce_53 = happyReduce 4 24 happyReduction_53
+#if __GLASGOW_HASKELL__ >= 710
+#endif
+happyReduce_53 = happyReduce 4# 20# happyReduction_53
 happyReduction_53 (_ `HappyStk`
-	(HappyAbsSyn26  happy_var_3) `HappyStk`
-	_ `HappyStk`
-	(HappyTerminal (TokenIdentifier happy_var_1)) `HappyStk`
-	happyRest)
-	 = HappyAbsSyn24
-		 ((happy_var_1, reverse happy_var_3)
-	) `HappyStk` happyRest
+        (HappyAbsSyn26  happy_var_3) `HappyStk`
+        _ `HappyStk`
+        (HappyTerminal (TokenIdentifier happy_var_1)) `HappyStk`
+        happyRest)
+         = HappyAbsSyn24
+                 ((happy_var_1, reverse happy_var_3)
+        ) `HappyStk` happyRest
 
-happyReduce_54 = happySpecReduce_2  25 happyReduction_54
+#if __GLASGOW_HASKELL__ >= 710
+#endif
+happyReduce_54 = happySpecReduce_2  21# happyReduction_54
 happyReduction_54 (HappyAbsSyn17  happy_var_2)
-	_
-	 =  HappyAbsSyn25
-		 (happy_var_2
-	)
+        _
+         =  HappyAbsSyn25
+                 (happy_var_2
+        )
 happyReduction_54 _ _  = notHappyAtAll 
 
-happyReduce_55 = happySpecReduce_1  25 happyReduction_55
+#if __GLASGOW_HASKELL__ >= 710
+#endif
+happyReduce_55 = happySpecReduce_1  21# happyReduction_55
 happyReduction_55 (HappyAbsSyn17  happy_var_1)
-	 =  HappyAbsSyn25
-		 (happy_var_1
-	)
+         =  HappyAbsSyn25
+                 (happy_var_1
+        )
 happyReduction_55 _  = notHappyAtAll 
 
-happyReduce_56 = happySpecReduce_0  26 happyReduction_56
+#if __GLASGOW_HASKELL__ >= 710
+#endif
+happyReduce_56 = happySpecReduce_0  22# happyReduction_56
 happyReduction_56  =  HappyAbsSyn26
-		 ([]
-	)
+                 ([]
+        )
 
-happyReduce_57 = happySpecReduce_1  26 happyReduction_57
+#if __GLASGOW_HASKELL__ >= 710
+#endif
+happyReduce_57 = happySpecReduce_1  22# happyReduction_57
 happyReduction_57 (HappyAbsSyn25  happy_var_1)
-	 =  HappyAbsSyn26
-		 ([happy_var_1]
-	)
+         =  HappyAbsSyn26
+                 ([happy_var_1]
+        )
 happyReduction_57 _  = notHappyAtAll 
 
-happyReduce_58 = happySpecReduce_3  26 happyReduction_58
+#if __GLASGOW_HASKELL__ >= 710
+#endif
+happyReduce_58 = happySpecReduce_3  22# happyReduction_58
 happyReduction_58 (HappyAbsSyn25  happy_var_3)
-	_
-	(HappyAbsSyn26  happy_var_1)
-	 =  HappyAbsSyn26
-		 (happy_var_3 : happy_var_1
-	)
+        _
+        (HappyAbsSyn26  happy_var_1)
+         =  HappyAbsSyn26
+                 (happy_var_3 : happy_var_1
+        )
 happyReduction_58 _ _ _  = notHappyAtAll 
 
-happyReduce_59 = happySpecReduce_1  27 happyReduction_59
+#if __GLASGOW_HASKELL__ >= 710
+#endif
+happyReduce_59 = happySpecReduce_1  23# happyReduction_59
 happyReduction_59 (HappyTerminal (TokenIdentifier happy_var_1))
-	 =  HappyAbsSyn27
-		 (happy_var_1 :| []
-	)
+         =  HappyAbsSyn27
+                 (happy_var_1 :| []
+        )
 happyReduction_59 _  = notHappyAtAll 
 
-happyReduce_60 = happySpecReduce_3  27 happyReduction_60
+#if __GLASGOW_HASKELL__ >= 710
+#endif
+happyReduce_60 = happySpecReduce_3  23# happyReduction_60
 happyReduction_60 (HappyTerminal (TokenIdentifier happy_var_3))
-	_
-	(HappyAbsSyn27  happy_var_1)
-	 =  HappyAbsSyn27
-		 (happy_var_3 <| happy_var_1
-	)
+        _
+        (HappyAbsSyn27  happy_var_1)
+         =  HappyAbsSyn27
+                 (happy_var_3 <| happy_var_1
+        )
 happyReduction_60 _ _ _  = notHappyAtAll 
 
-happyReduce_61 = happySpecReduce_1  28 happyReduction_61
+#if __GLASGOW_HASKELL__ >= 710
+#endif
+happyReduce_61 = happySpecReduce_1  24# happyReduction_61
 happyReduction_61 (HappyTerminal (TokenIdentifier happy_var_1))
-	 =  HappyAbsSyn28
-		 (happy_var_1
-	)
+         =  HappyAbsSyn28
+                 (happy_var_1
+        )
 happyReduction_61 _  = notHappyAtAll 
 
-happyReduce_62 = happySpecReduce_1  29 happyReduction_62
+#if __GLASGOW_HASKELL__ >= 710
+#endif
+happyReduce_62 = happySpecReduce_1  25# happyReduction_62
 happyReduction_62 (HappyTerminal (TokenIdentifier happy_var_1))
-	 =  HappyAbsSyn29
-		 (happy_var_1 :| []
-	)
+         =  HappyAbsSyn29
+                 (happy_var_1 :| []
+        )
 happyReduction_62 _  = notHappyAtAll 
 
-happyReduce_63 = happySpecReduce_3  29 happyReduction_63
+#if __GLASGOW_HASKELL__ >= 710
+#endif
+happyReduce_63 = happySpecReduce_3  25# happyReduction_63
 happyReduction_63 _
-	_
-	(HappyTerminal (TokenIdentifier happy_var_1))
-	 =  HappyAbsSyn29
-		 (happy_var_1 :| []
-	)
+        _
+        (HappyTerminal (TokenIdentifier happy_var_1))
+         =  HappyAbsSyn29
+                 (happy_var_1 :| []
+        )
 happyReduction_63 _ _ _  = notHappyAtAll 
 
-happyReduce_64 = happySpecReduce_3  29 happyReduction_64
+#if __GLASGOW_HASKELL__ >= 710
+#endif
+happyReduce_64 = happySpecReduce_3  25# happyReduction_64
 happyReduction_64 (HappyTerminal (TokenIdentifier happy_var_3))
-	_
-	(HappyAbsSyn29  happy_var_1)
-	 =  HappyAbsSyn29
-		 (happy_var_3 <| happy_var_1
-	)
+        _
+        (HappyAbsSyn29  happy_var_1)
+         =  HappyAbsSyn29
+                 (happy_var_3 <| happy_var_1
+        )
 happyReduction_64 _ _ _  = notHappyAtAll 
 
-happyReduce_65 = happyReduce 5 29 happyReduction_65
+#if __GLASGOW_HASKELL__ >= 710
+#endif
+happyReduce_65 = happyReduce 5# 25# happyReduction_65
 happyReduction_65 (_ `HappyStk`
-	_ `HappyStk`
-	(HappyTerminal (TokenIdentifier happy_var_3)) `HappyStk`
-	_ `HappyStk`
-	(HappyAbsSyn29  happy_var_1) `HappyStk`
-	happyRest)
-	 = HappyAbsSyn29
-		 (happy_var_3 <| happy_var_1
-	) `HappyStk` happyRest
+        _ `HappyStk`
+        (HappyTerminal (TokenIdentifier happy_var_3)) `HappyStk`
+        _ `HappyStk`
+        (HappyAbsSyn29  happy_var_1) `HappyStk`
+        happyRest)
+         = HappyAbsSyn29
+                 (happy_var_3 <| happy_var_1
+        ) `HappyStk` happyRest
 
-happyReduce_66 = happySpecReduce_1  30 happyReduction_66
+#if __GLASGOW_HASKELL__ >= 710
+#endif
+happyReduce_66 = happySpecReduce_1  26# happyReduction_66
 happyReduction_66 (HappyAbsSyn31  happy_var_1)
-	 =  HappyAbsSyn30
-		 (Number happy_var_1
-	)
+         =  HappyAbsSyn30
+                 (Number happy_var_1
+        )
 happyReduction_66 _  = notHappyAtAll 
 
-happyReduce_67 = happySpecReduce_3  30 happyReduction_67
+#if __GLASGOW_HASKELL__ >= 710
+#endif
+happyReduce_67 = happySpecReduce_3  26# happyReduction_67
 happyReduction_67 _
-	_
-	(HappyAbsSyn31  happy_var_1)
-	 =  HappyAbsSyn30
-		 (Number happy_var_1
-	)
+        _
+        (HappyAbsSyn31  happy_var_1)
+         =  HappyAbsSyn30
+                 (Number happy_var_1
+        )
 happyReduction_67 _ _ _  = notHappyAtAll 
 
-happyReduce_68 = happySpecReduce_1  30 happyReduction_68
+#if __GLASGOW_HASKELL__ >= 710
+#endif
+happyReduce_68 = happySpecReduce_1  26# happyReduction_68
 happyReduction_68 (HappyTerminal (TokenString happy_var_1))
-	 =  HappyAbsSyn30
-		 (Str happy_var_1
-	)
+         =  HappyAbsSyn30
+                 (Str happy_var_1
+        )
 happyReduction_68 _  = notHappyAtAll 
 
-happyReduce_69 = happySpecReduce_3  30 happyReduction_69
+#if __GLASGOW_HASKELL__ >= 710
+#endif
+happyReduce_69 = happySpecReduce_3  26# happyReduction_69
 happyReduction_69 _
-	_
-	(HappyTerminal (TokenString happy_var_1))
-	 =  HappyAbsSyn30
-		 (Str happy_var_1
-	)
+        _
+        (HappyTerminal (TokenString happy_var_1))
+         =  HappyAbsSyn30
+                 (Str happy_var_1
+        )
 happyReduction_69 _ _ _  = notHappyAtAll 
 
-happyReduce_70 = happySpecReduce_1  30 happyReduction_70
+#if __GLASGOW_HASKELL__ >= 710
+#endif
+happyReduce_70 = happySpecReduce_1  26# happyReduction_70
 happyReduction_70 _
-	 =  HappyAbsSyn30
-		 (Number 1
-	)
+         =  HappyAbsSyn30
+                 (Number 1
+        )
 
-happyReduce_71 = happySpecReduce_3  30 happyReduction_71
+#if __GLASGOW_HASKELL__ >= 710
+#endif
+happyReduce_71 = happySpecReduce_3  26# happyReduction_71
 happyReduction_71 _
-	_
-	_
-	 =  HappyAbsSyn30
-		 (Number 1
-	)
+        _
+        _
+         =  HappyAbsSyn30
+                 (Number 1
+        )
 
-happyReduce_72 = happySpecReduce_1  30 happyReduction_72
+#if __GLASGOW_HASKELL__ >= 710
+#endif
+happyReduce_72 = happySpecReduce_1  26# happyReduction_72
 happyReduction_72 _
-	 =  HappyAbsSyn30
-		 (Number 0
-	)
+         =  HappyAbsSyn30
+                 (Number 0
+        )
 
-happyReduce_73 = happySpecReduce_3  30 happyReduction_73
+#if __GLASGOW_HASKELL__ >= 710
+#endif
+happyReduce_73 = happySpecReduce_3  26# happyReduction_73
 happyReduction_73 _
-	_
-	_
-	 =  HappyAbsSyn30
-		 (Number 0
-	)
+        _
+        _
+         =  HappyAbsSyn30
+                 (Number 0
+        )
 
-happyReduce_74 = happySpecReduce_1  31 happyReduction_74
+#if __GLASGOW_HASKELL__ >= 710
+#endif
+happyReduce_74 = happySpecReduce_1  27# happyReduction_74
 happyReduction_74 (HappyTerminal (TokenHex happy_var_1))
-	 =  HappyAbsSyn31
-		 ((read happy_var_1)
-	)
+         =  HappyAbsSyn31
+                 ((read happy_var_1)
+        )
 happyReduction_74 _  = notHappyAtAll 
 
-happyReduce_75 = happySpecReduce_1  31 happyReduction_75
+#if __GLASGOW_HASKELL__ >= 710
+#endif
+happyReduce_75 = happySpecReduce_1  27# happyReduction_75
 happyReduction_75 (HappyTerminal (TokenDecimal happy_var_1))
-	 =  HappyAbsSyn31
-		 ((read happy_var_1)
-	)
+         =  HappyAbsSyn31
+                 ((read happy_var_1)
+        )
 happyReduction_75 _  = notHappyAtAll 
 
+#if __GLASGOW_HASKELL__ >= 710
+#endif
+happyReduce_76 = happySpecReduce_1  28# happyReduction_76
+happyReduction_76 (HappyTerminal (TokenString happy_var_1))
+         =  HappyAbsSyn32
+                 (happy_var_1
+        )
+happyReduction_76 _  = notHappyAtAll 
+
+#if __GLASGOW_HASKELL__ >= 710
+#endif
+happyReduce_77 = happySpecReduce_1  28# happyReduction_77
+happyReduction_77 (HappyTerminal (TokenHex happy_var_1))
+         =  HappyAbsSyn32
+                 (happy_var_1
+        )
+happyReduction_77 _  = notHappyAtAll 
+
 happyNewToken action sts stk [] =
-	action 60 60 notHappyAtAll (HappyState action) sts stk []
+        happyDoAction 29# notHappyAtAll action sts stk []
 
 happyNewToken action sts stk (tk:tks) =
-	let cont i = action i i tk (HappyState action) sts stk tks in
-	case tk of {
-	TokenLCurl -> cont 32;
-	TokenRCurl -> cont 33;
-	TokenLPar -> cont 34;
-	TokenRPar -> cont 35;
-	TokenArrow -> cont 36;
-	TokenColonEq -> cont 37;
-	TokenComma -> cont 38;
-	TokenColon -> cont 39;
-	TokenFunction -> cont 40;
-	TokenLet -> cont 41;
-	TokenIf -> cont 42;
-	TokenSwitch -> cont 43;
-	TokenCase -> cont 44;
-	TokenDefault -> cont 45;
-	TokenFor -> cont 46;
-	TokenBreak -> cont 47;
-	TokenContinue -> cont 48;
-	TokenLeave -> cont 49;
-	TokenTrue -> cont 50;
-	TokenFalse -> cont 51;
-	TokenIdentifier happy_dollar_dollar -> cont 52;
-	TokenString happy_dollar_dollar -> cont 53;
-	TokenHex happy_dollar_dollar -> cont 54;
-	TokenDecimal happy_dollar_dollar -> cont 55;
-	TokenInlineComment happy_dollar_dollar -> cont 56;
-	TokenMultilineComment happy_dollar_dollar -> cont 57;
-	TokenObject -> cont 58;
-	TokenCode -> cont 59;
-	_ -> happyError' ((tk:tks), [])
-	}
+        let cont i = happyDoAction i tk action sts stk tks in
+        case tk of {
+        TokenLCurl -> cont 1#;
+        TokenRCurl -> cont 2#;
+        TokenLPar -> cont 3#;
+        TokenRPar -> cont 4#;
+        TokenArrow -> cont 5#;
+        TokenColonEq -> cont 6#;
+        TokenComma -> cont 7#;
+        TokenColon -> cont 8#;
+        TokenFunction -> cont 9#;
+        TokenLet -> cont 10#;
+        TokenIf -> cont 11#;
+        TokenSwitch -> cont 12#;
+        TokenCase -> cont 13#;
+        TokenDefault -> cont 14#;
+        TokenFor -> cont 15#;
+        TokenBreak -> cont 16#;
+        TokenContinue -> cont 17#;
+        TokenLeave -> cont 18#;
+        TokenTrue -> cont 19#;
+        TokenFalse -> cont 20#;
+        TokenIdentifier happy_dollar_dollar -> cont 21#;
+        TokenString happy_dollar_dollar -> cont 22#;
+        TokenHex happy_dollar_dollar -> cont 23#;
+        TokenDecimal happy_dollar_dollar -> cont 24#;
+        TokenInlineComment happy_dollar_dollar -> cont 25#;
+        TokenMultilineComment happy_dollar_dollar -> cont 26#;
+        TokenObject -> cont 27#;
+        TokenCode -> cont 28#;
+        _ -> happyError' ((tk:tks), [])
+        }
 
-happyError_ explist 60 tk tks = happyError' (tks, explist)
+happyError_ explist 29# tk tks = happyError' (tks, explist)
 happyError_ explist _ tk tks = happyError' ((tk:tks), explist)
 
 newtype HappyIdentity a = HappyIdentity a
@@ -1323,7 +1031,7 @@ happyReturn1 = \a tks -> (Prelude.return) a
 happyError' :: () => ([(Token)], [Prelude.String]) -> HappyIdentity a
 happyError' = HappyIdentity Prelude.. (\(tokens, _) -> parseError tokens)
 calc tks = happyRunIdentity happySomeParser where
- happySomeParser = happyThen (happyParse action_0 tks) (\x -> case x of {HappyAbsSyn4 z -> happyReturn z; _other -> notHappyAtAll })
+ happySomeParser = happyThen (happyParse 0# tks) (\x -> case x of {HappyAbsSyn4 z -> happyReturn z; _other -> notHappyAtAll })
 
 happySeq = happyDontSeq
 
@@ -1336,90 +1044,53 @@ uncurry3 f (x, y, z) = f x y z
 
 uncurry4 :: (a -> b -> c -> d -> e) -> (a, b, c, d) -> e
 uncurry4 f (w, x, y, z) = f w x y z
-{-# LINE 1 "templates/GenericTemplate.hs" #-}
 -- $Id: GenericTemplate.hs,v 1.26 2005/01/14 14:47:22 simonmar Exp $
 
-
-
-
-
-
-
-
-
-
-
-
-
-
-
-
-
-
-
-
-
-
-
-
-
-
-
-
-
-
-
-
-
-
-
-
-
-
-
-
-
-
-data Happy_IntList = HappyCons Prelude.Int Happy_IntList
-
-
-
-
-
-
-
-
-
-
-
-
-
-
-
-
-
-
-
-
-
-
-
-
-
-
-
-
-
-
-
-
-
-
-
-
-
-
-
+#if !defined(__GLASGOW_HASKELL__)
+#  error This code isn't being built with GHC.
+#endif
+
+-- Get WORDS_BIGENDIAN (if defined)
+#include "MachDeps.h"
+
+-- Do not remove this comment. Required to fix CPP parsing when using GCC and a clang-compiled alex.
+#if __GLASGOW_HASKELL__ > 706
+#  define LT(n,m) ((Happy_GHC_Exts.tagToEnum# (n Happy_GHC_Exts.<# m)) :: Prelude.Bool)
+#  define GTE(n,m) ((Happy_GHC_Exts.tagToEnum# (n Happy_GHC_Exts.>=# m)) :: Prelude.Bool)
+#  define EQ(n,m) ((Happy_GHC_Exts.tagToEnum# (n Happy_GHC_Exts.==# m)) :: Prelude.Bool)
+#else
+#  define LT(n,m) (n Happy_GHC_Exts.<# m)
+#  define GTE(n,m) (n Happy_GHC_Exts.>=# m)
+#  define EQ(n,m) (n Happy_GHC_Exts.==# m)
+#endif
+#define PLUS(n,m) (n Happy_GHC_Exts.+# m)
+#define MINUS(n,m) (n Happy_GHC_Exts.-# m)
+#define TIMES(n,m) (n Happy_GHC_Exts.*# m)
+#define NEGATE(n) (Happy_GHC_Exts.negateInt# (n))
+
+type Happy_Int = Happy_GHC_Exts.Int#
+data Happy_IntList = HappyCons Happy_Int Happy_IntList
+
+#define ERROR_TOK 0#
+
+#if defined(HAPPY_COERCE)
+#  define GET_ERROR_TOKEN(x)  (case Happy_GHC_Exts.unsafeCoerce# x of { (Happy_GHC_Exts.I# i) -> i })
+#  define MK_ERROR_TOKEN(i)   (Happy_GHC_Exts.unsafeCoerce# (Happy_GHC_Exts.I# i))
+#  define MK_TOKEN(x)         (happyInTok (x))
+#else
+#  define GET_ERROR_TOKEN(x)  (case x of { HappyErrorToken (Happy_GHC_Exts.I# i) -> i })
+#  define MK_ERROR_TOKEN(i)   (HappyErrorToken (Happy_GHC_Exts.I# i))
+#  define MK_TOKEN(x)         (HappyTerminal (x))
+#endif
+
+#if defined(HAPPY_DEBUG)
+#  define DEBUG_TRACE(s)    (happyTrace (s)) $
+happyTrace string expr = Happy_System_IO_Unsafe.unsafePerformIO $ do
+    Happy_System_IO.hPutStr Happy_System_IO.stderr string
+    return expr
+#else
+#  define DEBUG_TRACE(s)    {- nothing -}
+#endif
 
 infixr 9 `HappyStk`
 data HappyStk a = HappyStk a (HappyStk a)
@@ -1435,184 +1106,175 @@ happyParse start_state = happyNewToken start_state notHappyAtAll notHappyAtAll
 -- If the current token is ERROR_TOK, it means we've just accepted a partial
 -- parse (a %partial parser).  We must ignore the saved token on the top of
 -- the stack in this case.
-happyAccept (1) tk st sts (_ `HappyStk` ans `HappyStk` _) =
+happyAccept ERROR_TOK tk st sts (_ `HappyStk` ans `HappyStk` _) =
         happyReturn1 ans
-happyAccept j tk st sts (HappyStk ans _) = 
-         (happyReturn1 ans)
+happyAccept j tk st sts (HappyStk ans _) =
+        (happyTcHack j (happyTcHack st)) (happyReturn1 ans)
 
 -----------------------------------------------------------------------------
 -- Arrays only: do the next action
 
+happyDoAction i tk st =
+  DEBUG_TRACE("state: " ++ show (Happy_GHC_Exts.I# st) ++
+              ",\ttoken: " ++ show (Happy_GHC_Exts.I# i) ++
+              ",\taction: ")
+  case happyDecodeAction (happyNextAction i st) of
+    HappyFail             -> DEBUG_TRACE("failing.\n")
+                             happyFail (happyExpListPerState (Happy_GHC_Exts.I# st)) i tk st
+    HappyAccept           -> DEBUG_TRACE("accept.\n")
+                             happyAccept i tk st
+    HappyReduce rule      -> DEBUG_TRACE("reduce (rule " ++ show (Happy_GHC_Exts.I# rule) ++ ")")
+                             (happyReduceArr Happy_Data_Array.! (Happy_GHC_Exts.I# rule)) i tk st
+    HappyShift  new_state -> DEBUG_TRACE("shift, enter state " ++ show (Happy_GHC_Exts.I# new_state) ++ "\n")
+                             happyShift new_state i tk st
 
+{-# INLINE happyNextAction #-}
+happyNextAction i st = case happyIndexActionTable i st of
+  Just (Happy_GHC_Exts.I# act) -> act
+  Nothing                      -> happyIndexOffAddr happyDefActions st
 
+{-# INLINE happyIndexActionTable #-}
+happyIndexActionTable i st
+  | GTE(off, 0#), EQ(happyIndexOffAddr happyCheck off, i)
+  = Prelude.Just (Happy_GHC_Exts.I# (happyIndexOffAddr happyTable off))
+  | otherwise
+  = Prelude.Nothing
+  where
+    off = PLUS(happyIndexOffAddr happyActOffsets st, i)
 
+data HappyAction
+  = HappyFail
+  | HappyAccept
+  | HappyReduce Happy_Int -- rule number
+  | HappyShift Happy_Int  -- new state
 
+{-# INLINE happyDecodeAction #-}
+happyDecodeAction :: Happy_Int -> HappyAction
+happyDecodeAction  0#                        = HappyFail
+happyDecodeAction -1#                        = HappyAccept
+happyDecodeAction action | LT(action, 0#)    = HappyReduce NEGATE(PLUS(action, 1#))
+                         | otherwise         = HappyShift MINUS(action, 1#)
 
+{-# INLINE happyIndexGotoTable #-}
+happyIndexGotoTable nt st = happyIndexOffAddr happyTable off
+  where
+    off = PLUS(happyIndexOffAddr happyGotoOffsets st, nt)
 
-
-
-
-
-
-
-
-
-
-
-
-
-
-
-
-
-
-
-
-
-
-
-
-
-
-
-
-
-
-
-
-
-
-
-indexShortOffAddr arr off = arr Happy_Data_Array.! off
-
+{-# INLINE happyIndexOffAddr #-}
+happyIndexOffAddr :: HappyAddr -> Happy_Int -> Happy_Int
+happyIndexOffAddr (HappyA# arr) off =
+#if __GLASGOW_HASKELL__ >= 901
+  Happy_GHC_Exts.int32ToInt# -- qualified import because it doesn't exist on older GHC's
+#endif
+#ifdef WORDS_BIGENDIAN
+  -- The CI of `alex` tests this code path
+  (Happy_GHC_Exts.word32ToInt32# (Happy_GHC_Exts.wordToWord32# (Happy_GHC_Exts.byteSwap32# (Happy_GHC_Exts.word32ToWord# (Happy_GHC_Exts.int32ToWord32#
+#endif
+  (Happy_GHC_Exts.indexInt32OffAddr# arr off)
+#ifdef WORDS_BIGENDIAN
+  )))))
+#endif
 
 {-# INLINE happyLt #-}
-happyLt x y = (x Prelude.< y)
-
-
-
-
-
+happyLt x y = LT(x,y)
 
 readArrayBit arr bit =
-    Bits.testBit (indexShortOffAddr arr (bit `Prelude.div` 16)) (bit `Prelude.mod` 16)
+    Bits.testBit (Happy_GHC_Exts.I# (happyIndexOffAddr arr ((unbox_int bit) `Happy_GHC_Exts.iShiftRA#` 5#))) (bit `Prelude.mod` 32)
+  where unbox_int (Happy_GHC_Exts.I# x) = x
 
-
-
-
-
-
------------------------------------------------------------------------------
--- HappyState data type (not arrays)
-
-
-
-newtype HappyState b c = HappyState
-        (Prelude.Int ->                    -- token number
-         Prelude.Int ->                    -- token number (yes, again)
-         b ->                           -- token semantic value
-         HappyState b c ->              -- current state
-         [HappyState b c] ->            -- state stack
-         c)
-
-
+data HappyAddr = HappyA# Happy_GHC_Exts.Addr#
 
 -----------------------------------------------------------------------------
 -- Shifting a token
 
-happyShift new_state (1) tk st sts stk@(x `HappyStk` _) =
-     let i = (case x of { HappyErrorToken (i) -> i }) in
---     trace "shifting the error token" $
-     new_state i i tk (HappyState (new_state)) ((st):(sts)) (stk)
+happyShift new_state ERROR_TOK tk st sts stk@(x `HappyStk` _) =
+     let i = GET_ERROR_TOKEN(x) in
+-- trace "shifting the error token" $
+     happyDoAction i tk new_state (HappyCons st sts) stk
 
 happyShift new_state i tk st sts stk =
-     happyNewToken new_state ((st):(sts)) ((HappyTerminal (tk))`HappyStk`stk)
+     happyNewToken new_state (HappyCons st sts) (MK_TOKEN(tk) `HappyStk` stk)
 
 -- happyReduce is specialised for the common cases.
 
-happySpecReduce_0 i fn (1) tk st sts stk
-     = happyFail [] (1) tk st sts stk
-happySpecReduce_0 nt fn j tk st@((HappyState (action))) sts stk
-     = action nt j tk st ((st):(sts)) (fn `HappyStk` stk)
+happySpecReduce_0 i fn ERROR_TOK tk st sts stk
+     = happyFail [] ERROR_TOK tk st sts stk
+happySpecReduce_0 nt fn j tk st sts stk
+     = happyGoto nt j tk st (HappyCons st sts) (fn `HappyStk` stk)
 
-happySpecReduce_1 i fn (1) tk st sts stk
-     = happyFail [] (1) tk st sts stk
-happySpecReduce_1 nt fn j tk _ sts@(((st@(HappyState (action))):(_))) (v1`HappyStk`stk')
+happySpecReduce_1 i fn ERROR_TOK tk st sts stk
+     = happyFail [] ERROR_TOK tk st sts stk
+happySpecReduce_1 nt fn j tk _ sts@(HappyCons st _) (v1 `HappyStk` stk')
      = let r = fn v1 in
-       happySeq r (action nt j tk st sts (r `HappyStk` stk'))
+       happySeq r (happyGoto nt j tk st sts (r `HappyStk` stk'))
 
-happySpecReduce_2 i fn (1) tk st sts stk
-     = happyFail [] (1) tk st sts stk
-happySpecReduce_2 nt fn j tk _ ((_):(sts@(((st@(HappyState (action))):(_))))) (v1`HappyStk`v2`HappyStk`stk')
+happySpecReduce_2 i fn ERROR_TOK tk st sts stk
+     = happyFail [] ERROR_TOK tk st sts stk
+happySpecReduce_2 nt fn j tk _
+  (HappyCons _ sts@(HappyCons st _))
+  (v1 `HappyStk` v2 `HappyStk` stk')
      = let r = fn v1 v2 in
-       happySeq r (action nt j tk st sts (r `HappyStk` stk'))
+       happySeq r (happyGoto nt j tk st sts (r `HappyStk` stk'))
 
-happySpecReduce_3 i fn (1) tk st sts stk
-     = happyFail [] (1) tk st sts stk
-happySpecReduce_3 nt fn j tk _ ((_):(((_):(sts@(((st@(HappyState (action))):(_))))))) (v1`HappyStk`v2`HappyStk`v3`HappyStk`stk')
+happySpecReduce_3 i fn ERROR_TOK tk st sts stk
+     = happyFail [] ERROR_TOK tk st sts stk
+happySpecReduce_3 nt fn j tk _
+  (HappyCons _ (HappyCons _ sts@(HappyCons st _)))
+  (v1 `HappyStk` v2 `HappyStk` v3 `HappyStk` stk')
      = let r = fn v1 v2 v3 in
-       happySeq r (action nt j tk st sts (r `HappyStk` stk'))
+       happySeq r (happyGoto nt j tk st sts (r `HappyStk` stk'))
 
-happyReduce k i fn (1) tk st sts stk
-     = happyFail [] (1) tk st sts stk
+happyReduce k i fn ERROR_TOK tk st sts stk
+     = happyFail [] ERROR_TOK tk st sts stk
 happyReduce k nt fn j tk st sts stk
-     = case happyDrop (k Prelude.- ((1) :: Prelude.Int)) sts of
-         sts1@(((st1@(HappyState (action))):(_))) ->
-                let r = fn stk in  -- it doesn't hurt to always seq here...
-                happyDoSeq r (action nt j tk st1 sts1 r)
+     = case happyDrop MINUS(k,(1# :: Happy_Int)) sts of
+         sts1@(HappyCons st1 _) ->
+                let r = fn stk in -- it doesn't hurt to always seq here...
+                happyDoSeq r (happyGoto nt j tk st1 sts1 r)
 
-happyMonadReduce k nt fn (1) tk st sts stk
-     = happyFail [] (1) tk st sts stk
+happyMonadReduce k nt fn ERROR_TOK tk st sts stk
+     = happyFail [] ERROR_TOK tk st sts stk
 happyMonadReduce k nt fn j tk st sts stk =
-      case happyDrop k ((st):(sts)) of
-        sts1@(((st1@(HappyState (action))):(_))) ->
+      case happyDrop k (HappyCons st sts) of
+        sts1@(HappyCons st1 _) ->
           let drop_stk = happyDropStk k stk in
-          happyThen1 (fn stk tk) (\r -> action nt j tk st1 sts1 (r `HappyStk` drop_stk))
+          happyThen1 (fn stk tk)
+                     (\r -> happyGoto nt j tk st1 sts1 (r `HappyStk` drop_stk))
 
-happyMonad2Reduce k nt fn (1) tk st sts stk
-     = happyFail [] (1) tk st sts stk
+happyMonad2Reduce k nt fn ERROR_TOK tk st sts stk
+     = happyFail [] ERROR_TOK tk st sts stk
 happyMonad2Reduce k nt fn j tk st sts stk =
-      case happyDrop k ((st):(sts)) of
-        sts1@(((st1@(HappyState (action))):(_))) ->
-         let drop_stk = happyDropStk k stk
-
-
-
-
-
-             _ = nt :: Prelude.Int
-             new_state = action
-
+      case happyDrop k (HappyCons st sts) of
+        sts1@(HappyCons st1 _) ->
+          let drop_stk = happyDropStk k stk
+              off = happyAdjustOffset (happyIndexOffAddr happyGotoOffsets st1)
+              off_i = PLUS(off, nt)
+              new_state = happyIndexOffAddr happyTable off_i
           in
-          happyThen1 (fn stk tk) (\r -> happyNewToken new_state sts1 (r `HappyStk` drop_stk))
+            happyThen1 (fn stk tk)
+                       (\r -> happyNewToken new_state sts1 (r `HappyStk` drop_stk))
 
-happyDrop (0) l = l
-happyDrop n ((_):(t)) = happyDrop (n Prelude.- ((1) :: Prelude.Int)) t
+happyDrop 0# l               = l
+happyDrop n  (HappyCons _ t) = happyDrop MINUS(n,(1# :: Happy_Int)) t
 
-happyDropStk (0) l = l
-happyDropStk n (x `HappyStk` xs) = happyDropStk (n Prelude.- ((1)::Prelude.Int)) xs
+happyDropStk 0# l                 = l
+happyDropStk n  (x `HappyStk` xs) = happyDropStk MINUS(n,(1#::Happy_Int)) xs
 
 -----------------------------------------------------------------------------
 -- Moving to a new state after a reduction
 
-
-
-
-
-
-
-
-
-happyGoto action j tk st = action j j tk (HappyState action)
-
+happyGoto nt j tk st =
+   DEBUG_TRACE(", goto state " ++ show (Happy_GHC_Exts.I# new_state) ++ "\n")
+   happyDoAction j tk new_state
+  where new_state = happyIndexGotoTable nt st
 
 -----------------------------------------------------------------------------
 -- Error recovery (ERROR_TOK is the error token)
 
 -- parse error if we are in recovery and we fail again
-happyFail explist (1) tk old_st _ stk@(x `HappyStk` _) =
-     let i = (case x of { HappyErrorToken (i) -> i }) in
---      trace "failing" $ 
+happyFail explist ERROR_TOK tk old_st _ stk@(x `HappyStk` _) =
+     let i = GET_ERROR_TOKEN(x) in
+--      trace "failing" $
         happyError_ explist i tk
 
 {-  We don't need state discarding for our restricted implementation of
@@ -1620,17 +1282,17 @@ happyFail explist (1) tk old_st _ stk@(x `HappyStk` _) =
     for now --SDM
 
 -- discard a state
-happyFail  ERROR_TOK tk old_st CONS(HAPPYSTATE(action),sts) 
-                                                (saved_tok `HappyStk` _ `HappyStk` stk) =
+happyFail  ERROR_TOK tk old_st (HappyCons action sts)
+                               (saved_tok `HappyStk` _ `HappyStk` stk) =
 --      trace ("discarding state, depth " ++ show (length stk))  $
-        DO_ACTION(action,ERROR_TOK,tk,sts,(saved_tok`HappyStk`stk))
+        happyDoAction ERROR_TOK tk action sts (saved_tok`HappyStk`stk)
 -}
 
 -- Enter error recovery: generate an error token,
 --                       save the old token and carry on.
-happyFail explist i tk (HappyState (action)) sts stk =
---      trace "entering error recovery" $
-        action (1) (1) tk (HappyState (action)) sts ((HappyErrorToken (i)) `HappyStk` stk)
+happyFail explist i tk action sts stk =
+-- trace "entering error recovery" $
+        happyDoAction ERROR_TOK tk action sts (MK_ERROR_TOKEN(i) `HappyStk` stk)
 
 -- Internal happy errors:
 
@@ -1640,14 +1302,12 @@ notHappyAtAll = Prelude.error "Internal Happy error\n"
 -----------------------------------------------------------------------------
 -- Hack to get the typechecker to accept our action functions
 
-
-
-
-
-
+happyTcHack :: Happy_Int -> a -> a
+happyTcHack x y = y
+{-# INLINE happyTcHack #-}
 
 -----------------------------------------------------------------------------
--- Seq-ing.  If the --strict flag is given, then Happy emits 
+-- Seq-ing.  If the --strict flag is given, then Happy emits
 --      happySeq = happyDoSeq
 -- otherwise it emits
 --      happySeq = happyDontSeq
@@ -1661,13 +1321,12 @@ happyDontSeq a b = b
 -- of deciding to inline happyGoto everywhere, which increases the size of
 -- the generated parser quite a bit.
 
-
-
-
-
-
-
-
+{-# NOINLINE happyDoAction #-}
+{-# NOINLINE happyTable #-}
+{-# NOINLINE happyCheck #-}
+{-# NOINLINE happyActOffsets #-}
+{-# NOINLINE happyGotoOffsets #-}
+{-# NOINLINE happyDefActions #-}
 
 {-# NOINLINE happyShift #-}
 {-# NOINLINE happySpecReduce_0 #-}
